adder specification

Arithmetic.v
@@ -37,20 +37,20 @@ Definition adder_cout_bexp : bexp := (3 ∧ (2 ⊻ 1)) ⊻ (2 ∧ 1).
 Input : var 0 : y
         var 1 : x
         var 2 : cin
-Output : z = cin ⊕ (x ⊕ y)
+Output : sum = cin ⊕ (x ⊕ y)
  *)
-Definition adder_z_bexp : bexp := 2 ⊻ (1 ⊻ 0).
+Definition adder_sum_bexp : bexp := 2 ⊻ (1 ⊻ 0).
 
 (*
 Input : var 0 : x
         var 1 : y
-Output : z = x ⊕ y
+Output : xor = x ⊕ y
 *)
 Definition xor_bexp : bexp := 0 ⊻ 1.
 
 (*
 Input : var 0 : x
-Output : z = x
+Output : x' = x
 *)
 Definition id_bexp : bexp := 0.
 
@@ -93,29 +93,29 @@ Lemma test_adder_cout_bexp_111 :
 ⌈ adder_cout_bexp | fun_of_bools [false; true; true; true] ⌉ = true.
 Proof. simpl. reflexivity. Qed.
 
-Lemma test_adder_z_bexp_000 : 
-⌈ adder_z_bexp | fun_of_bools [false; false; false] ⌉ = false.
+Lemma test_adder_sum_bexp_000 : 
+⌈ adder_sum_bexp | fun_of_bools [false; false; false] ⌉ = false.
 Proof. simpl. reflexivity. Qed.
-Lemma test_adder_z_bexp_001 : 
-⌈ adder_z_bexp | fun_of_bools [false; false; true] ⌉ = true.
+Lemma test_adder_sum_bexp_001 : 
+⌈ adder_sum_bexp | fun_of_bools [false; false; true] ⌉ = true.
 Proof. simpl. reflexivity. Qed.
-Lemma test_adder_z_bexp_010 : 
-⌈ adder_z_bexp | fun_of_bools [false; true; false] ⌉ = true.
+Lemma test_adder_sum_bexp_010 : 
+⌈ adder_sum_bexp | fun_of_bools [false; true; false] ⌉ = true.
 Proof. simpl. reflexivity. Qed.
-Lemma test_adder_z_bexp_011 : 
-⌈ adder_z_bexp | fun_of_bools [false; true; true] ⌉ = false.
+Lemma test_adder_sum_bexp_011 : 
+⌈ adder_sum_bexp | fun_of_bools [false; true; true] ⌉ = false.
 Proof. simpl. reflexivity. Qed.
-Lemma test_adder_z_bexp_100 : 
-⌈ adder_z_bexp | fun_of_bools [true; false; false] ⌉ = true.
+Lemma test_adder_sum_bexp_100 : 
+⌈ adder_sum_bexp | fun_of_bools [true; false; false] ⌉ = true.
 Proof. simpl. reflexivity. Qed.
-Lemma test_adder_z_bexp_101 : 
-⌈ adder_z_bexp | fun_of_bools [true; false; true] ⌉ = false.
+Lemma test_adder_sum_bexp_101 : 
+⌈ adder_sum_bexp | fun_of_bools [true; false; true] ⌉ = false.
 Proof. simpl. reflexivity. Qed.
-Lemma test_adder_z_bexp_110 : 
-⌈ adder_z_bexp | fun_of_bools [true; true; false] ⌉ = false.
+Lemma test_adder_sum_bexp_110 : 
+⌈ adder_sum_bexp | fun_of_bools [true; true; false] ⌉ = false.
 Proof. simpl. reflexivity. Qed.
-Lemma test_adder_z_bexp_111 : 
-⌈ adder_z_bexp | fun_of_bools [true; true; true] ⌉ = true.
+Lemma test_adder_sum_bexp_111 : 
+⌈ adder_sum_bexp | fun_of_bools [true; true; true] ⌉ = true.
 Proof. simpl. reflexivity. Qed.
 
 Close Scope bexp_scope.
@@ -127,15 +127,15 @@ Definition adder_cout_circ :=
   compile adder_cout_bexp (list_of_Qubits 4).
 Eval compute in adder_cout_circ.
 
-Definition adder_z_circ := compile adder_z_bexp (list_of_Qubits 3).
+Definition adder_sum_circ := compile adder_sum_bexp (list_of_Qubits 3).
 
 (* adder_cout circuit with pads, input type is ((4+n) ⨂ Qubit), Box ((5+n) ⨂ Qubit) ((5+n) ⨂ Qubit) *)
 Definition adder_cout_circ_with_pads (n : nat) :=
   compile adder_cout_bexp (list_of_Qubits (4+n)).
 
-(* adder_z circuit with pads, input type is ((3+n) ⨂ Qubit), Box ((4+n) ⨂ Qubit) ((4+n) ⨂ Qubit) *)
-Definition adder_z_circ_with_pads (n : nat) :=
-  compile adder_z_bexp (list_of_Qubits (3+n)).
+(* adder_sum circuit with pads, input type is ((3+n) ⨂ Qubit), Box ((4+n) ⨂ Qubit) ((4+n) ⨂ Qubit) *)
+Definition adder_sum_circ_with_pads (n : nat) :=
+  compile adder_sum_bexp (list_of_Qubits (3+n)).
 
 Definition calc_xor_circ :=
   compile xor_bexp (list_of_Qubits 2).
@@ -143,8 +143,6 @@ Definition calc_xor_circ :=
 Definition calc_id_circ := compile id_bexp (list_of_Qubits 1).
 
 Notation "'let_' ( p1 , p2 ) ← 'output' p3 ; c" := (letpair p1 p2 p3 c) (at level 12, right associativity) : circ_scope.
-Notation "'let_' p ← c1 ; c2" := (comp p c1 c2)
-                            (at level 12, right associativity) : circ_scope.
 
 Ltac compute_compile :=
   repeat (try unfold compile; simpl;
@@ -160,24 +158,38 @@ Proof.
   compute_compile.
  *)
 (*
-Derive p SuchThat (adder_z_circ = p) As h.
+Require Coq.derive.Derive.
+Derive p SuchThat (adder_sum_circ = p) As h.
 Proof.
-  unfold adder_z_circ; unfold adder_z_bexp.
-  compute_compile. Set Printing Implicit.
-*)
+  unfold adder_sum_circ; unfold adder_sum_bexp.
+  compute_compile. 
+  repeat (unfold comp; simpl). cbv.
+  
+  Check (output ∘ pair (qubit 1)). simpl_eq. show_goal. show_hyps. program_simpl. unfold compose. simpl.
+  unfold comp. Locate "∘". Check pair.
+Notation "'let_' p ← 'unbox' ( c1 ) ; c2" := (comp p c1 c2) (at level 12, right associativity) : circ_scope.
 
+(let_ (p8, p9)← output p7;
+                          comp p2'
+                            (comp x
+                               (let_ (p10, p11)← output p9;
+                                gate_ p' ← assert0 @ p10; (p', p11))
+                               (let_ (_, p')← output x; p')) (p8, p2'))
+  
+  let_ (z_2, out_z) ← unbox adder_z_circ (z_1, (y_1, (pair x_1 (pair cin_1 unit))));
+*)
 
 Definition calc_id_circ_with_pads (n : nat) := compile id_bexp (list_of_Qubits (1+n)).
 
 Lemma adder_cout_circ_WT : Typed_Box adder_cout_circ.
 Proof. apply compile_WT. Qed.
-Lemma adder_z_circ_WT : Typed_Box adder_z_circ.
+Lemma adder_sum_circ_WT : Typed_Box adder_sum_circ.
 Proof. apply compile_WT. Qed.
 Lemma adder_cout_circ_with_pads_WT : forall n,
   Typed_Box (adder_cout_circ_with_pads n).
 Proof. intros. apply compile_WT. Qed.
-Lemma adder_z_circ_with_pads_WT : forall n,
-  Typed_Box (adder_z_circ_with_pads n).
+Lemma adder_sum_circ_with_pads_WT : forall n,
+  Typed_Box (adder_sum_circ_with_pads n).
 Proof. intros. apply compile_WT. Qed.
 Lemma calc_xor_circ_WT : Typed_Box calc_xor_circ.
 Proof. apply compile_WT. Qed.
@@ -189,24 +201,28 @@ Proof. intros. apply compile_WT. Qed.
 
 Open Scope matrix_scope.
 
-Lemma adder_cout_circ_spec : forall (cout z y x cin : bool),
-⟦adder_cout_circ⟧ (bool_to_matrix cout ⊗ bools_to_matrix [z; y; x; cin])
-= bools_to_matrix ((cout ⊕ ⌈ adder_cout_bexp | fun_of_bools [z; y; x; cin] ⌉) :: [z; y; x; cin]).
+(* Specifications *)
+
+Definition calc_cout (cin x y : bool) : bool := (cin && (x ⊕ y)) ⊕ (x && y).
+Definition calc_sum (cin x y : bool) : bool := cin ⊕ (x ⊕ y).
+
+Lemma adder_cout_circ_spec : forall (cout sum y x cin : bool),
+⟦adder_cout_circ⟧ (bool_to_matrix cout ⊗ bools_to_matrix [sum; y; x; cin])
+= bools_to_matrix ((cout ⊕ (calc_cout cin x y)) :: [sum; y; x; cin]).
 Proof.
 intros.
 apply (compile_correct adder_cout_bexp (list_of_Qubits 4) 
-  (fun_of_bools [z; y; x; cin]) cout).
+  (fun_of_bools [sum; y; x; cin]) cout).
 repeat constructor.
 Qed.
 
-Lemma adder_z_circ_spec : forall (z y x cin : bool),
-⟦adder_z_circ⟧ (bool_to_matrix z ⊗ bools_to_matrix [y; x; cin])
-= bool_to_matrix (z ⊕ ⌈ adder_z_bexp | fun_of_bools [y; x; cin]⌉) ⊗ 
-  bools_to_matrix [y; x; cin].
+Lemma adder_sum_circ_spec : forall (sum y x cin : bool),
+⟦adder_sum_circ⟧ (bool_to_matrix sum ⊗ bools_to_matrix [y; x; cin])
+= bool_to_matrix (sum ⊕ (calc_sum cin x y)) ⊗  bools_to_matrix [y; x; cin].
 Proof.
 intros.
-apply (compile_correct adder_z_bexp [Some Qubit; Some Qubit; Some Qubit] 
-  (fun_of_bools [y; x; cin]) z).
+apply (compile_correct adder_sum_bexp (list_of_Qubits 3) 
+  (fun_of_bools [y; x; cin]) sum).
 repeat constructor.
 Qed.
 
@@ -220,13 +236,13 @@ apply (compile_correct adder_cout_bexp (list_of_Qubits (4+n)) (fun x => f (S x))
 repeat constructor.
 Qed.
 
-Lemma adder_z_circ_with_pads_spec : forall (n : nat) (f : Var -> bool),
-⟦adder_z_circ_with_pads n⟧ ((bool_to_matrix (f 0)) ⊗ (ctx_to_matrix (list_of_Qubits (3+n)) (fun x => f (S x))))
-= (bool_to_matrix ((f 0) ⊕ ⌈ adder_z_bexp | (fun x => f (S x)) ⌉)) ⊗ 
+Lemma adder_sum_circ_with_pads_spec : forall (n : nat) (f : Var -> bool),
+⟦adder_sum_circ_with_pads n⟧ ((bool_to_matrix (f 0)) ⊗ (ctx_to_matrix (list_of_Qubits (3+n)) (fun x => f (S x))))
+= (bool_to_matrix ((f 0) ⊕ ⌈ adder_sum_bexp | (fun x => f (S x)) ⌉)) ⊗ 
   (ctx_to_matrix (list_of_Qubits (3+n)) (fun x => f (S x))).
 Proof.
 intros.
-apply (compile_correct adder_z_bexp (list_of_Qubits (3+n)) (fun x => f (S x)) (f 0%nat)).
+apply (compile_correct adder_sum_bexp (list_of_Qubits (3+n)) (fun x => f (S x)) (f 0%nat)).
 repeat constructor.
 Qed.
 
@@ -241,12 +257,12 @@ repeat constructor.
 Qed.
 
 (* Proof of specification using matrix_denote : failed
-Lemma calc_xor_circ_spec_matrix : forall (x y z : bool),
-  ⟦xor_circ⟧ ((bool_to_matrix x) ⊗ (bool_to_matrix y) ⊗ (bool_to_matrix z))
-  = ((bool_to_matrix x) ⊗ (bool_to_matrix y) ⊗ (bool_to_matrix (x ⊕ y ⊕ z))).
+Lemma calc_xor_circ_spec_matrix : forall (x y sum : bool),
+  ⟦xor_circ⟧ ((bool_to_matrix x) ⊗ (bool_to_matrix y) ⊗ (bool_to_matrix sum))
+  = ((bool_to_matrix x) ⊗ (bool_to_matrix y) ⊗ (bool_to_matrix (x ⊕ y ⊕ sum))).
 Proof.
   matrix_denote. Msimpl.
-  destruct x, y, z; unfold bool_to_ket; simpl; Msimpl; solve_matrix. 
+  destruct x, y, sum; unfold bool_to_ket; simpl; Msimpl; solve_matrix. 
 Qed.
 *)
 
@@ -273,28 +289,45 @@ Qed.
 Close Scope matrix_scope.
 
 (*
-Input : (cout, (z, (y, (x, (cin, ())))))
-Output : (cout', (z', (y, (x, (cin, ())))))
+Input : (cout, (sum, (y, (x, (cin, ())))))
+Output : (cout', (sum', (y, (x, (cin, ())))))
+*)
+Definition carrier_circ_1 : Box (5 ⨂ Qubit) (5 ⨂ Qubit) := adder_cout_circ.
+
+(*
+Input : (cout, (sum, (y, (x, (cin, ())))))
+Output : (cout', (sum', (y, (x, (cin, ())))))
 *)
 Definition adder_circ_1 : Box (5 ⨂ Qubit) (5 ⨂ Qubit) := 
-  (id_circ ∥ adder_z_circ) ;; adder_cout_circ.
+  (id_circ ∥ adder_sum_circ) ;; adder_cout_circ.
 
 (*
 Require Coq.derive.Derive.
 Derive p SuchThat (adder_circ_1 = p) As h.
 Proof.
   unfold adder_circ_1.
-  unfold inPar; unfold inSeq.
-  unfold id_circ; unfold adder_z_circ; unfold adder_cout_circ.
-  unfold id_bexp; unfold adder_z_bexp; unfold adder_cout_bexp.
-  unfold compile. simpl.
-  unfold Symmetric.CNOT_at. simpl.
-*)
+  unfold adder_sum_circ; unfold adder_sum_bexp.
+  unfold adder_cout_circ; unfold adder_cout_bexp.
+  compute_compile. 
+ *)
 
+Local Obligation Tactic := program_simpl; try omega.
+Program Definition carrier_circ_1_with_pads (n : nat) : Box ((5+n) ⨂ Qubit) ((5+n) ⨂ Qubit)
+  := (adder_cout_circ_with_pads n).
+Next Obligation.
+  induction n.
+  - reflexivity.
+  - simpl. rewrite IHn. reflexivity.
+Defined.
+Next Obligation.
+  induction n.
+  - reflexivity.
+  - simpl. rewrite IHn. reflexivity.
+Defined.
 
 Local Obligation Tactic := program_simpl; try omega.
 Program Definition adder_circ_1_with_pads (n : nat) : Box ((5+n) ⨂ Qubit) ((5+n) ⨂ Qubit) := 
-  ((@id_circ Qubit) ∥ (adder_z_circ_with_pads n)) ;; 
+  ((@id_circ Qubit) ∥ (adder_sum_circ_with_pads n)) ;; 
   (adder_cout_circ_with_pads n).
 Next Obligation.
   induction n.
@@ -307,12 +340,26 @@ Next Obligation.
   - simpl. rewrite IHn. reflexivity.
 Defined.
 
+Lemma carrier_circ_1_WT : Typed_Box carrier_circ_1.
+Proof.
+  unfold carrier_circ_1.
+  apply adder_cout_circ_WT.
+Qed.
+
+Lemma carrier_circ_1_with_pads_WT : forall (n : nat),
+  Typed_Box (carrier_circ_1_with_pads n).
+Proof.
+  intros.
+  unfold carrier_circ_1_with_pads. simpl_eq.
+  apply adder_cout_circ_with_pads_WT.
+Qed.
+
 Lemma adder_circ_1_WT : Typed_Box adder_circ_1.
 Proof.
   apply inSeq_WT.
   - apply inPar_WT.
     + apply id_circ_WT.
-    + apply adder_z_circ_WT.
+    + apply adder_sum_circ_WT.
   - apply adder_cout_circ_WT.
 Qed.
 
@@ -324,26 +371,85 @@ Proof.
   apply inSeq_WT.
   - apply inPar_WT.
     + apply id_circ_WT.
-    +apply adder_z_circ_with_pads_WT.
+    +apply adder_sum_circ_with_pads_WT.
   - apply adder_cout_circ_with_pads_WT.
 Qed.
 
 Open Scope matrix_scope.
-Lemma adder_circ_1_spec : forall (cin x y z cout : bool),
-  ⟦adder_circ_1⟧ (ctx_to_matrix (list_of_Qubits 5) (fun_of_bools [cout; z; y; x; cin]))
-  = (ctx_to_matrix 
-      (list_of_Qubits 5) 
-      (fun_of_bools [cout ⊕ ⌈ adder_cout_bexp | fun_of_bools [z; y; x; cin] ⌉; 
-                         z ⊕ ⌈ adder_z_bexp | fun_of_bools [y; x; cin] ⌉; y; x; cin])).
+
+Lemma dim_eq_lemma_1 : forall n, (size_ctx (list_of_Qubits n )) = n.
+Proof.
+  induction n.
+  - reflexivity.
+  - simpl. unfold list_of_Qubits in IHn. rewrite IHn. reflexivity.
+Qed.
+Lemma dim_eq_lemma_2 : forall n (f : Var -> bool),
+    @length (Square 2) (ctx_to_mat_list (list_of_Qubits n) f) = n.
+Proof.
+  induction n.
+  - reflexivity.
+  - intros. simpl. rewrite IHn. reflexivity.
+Qed.
+Lemma dim_eq_lemma_3 : forall n, size_wtype (NTensor n Qubit) = n.
+Proof.
+  induction n.
+  - reflexivity.
+  - simpl. rewrite IHn. reflexivity.
+Qed.
+Lemma kron_eq_1 : forall {m n o p} m11 m12 m21 m22,
+                 m11 = m21 -> m12 = m22 -> @kron m n o p m11 m12 = @kron m n o p m21 m22.
+  intros. rewrite H. rewrite H0. reflexivity.
+Qed.
+Lemma big_kron_eq_1 : forall n f1 f2,
+    (forall x, f1 x = f2 x) ->
+    ⨂ ctx_to_mat_list (list_of_Qubits n) f1 = ⨂ ctx_to_mat_list (list_of_Qubits n) f2.
+Proof.
+  induction n.
+  - intros. simpl. reflexivity.
+  - intros. simpl. unfold list_of_Qubits in IHn.
+    rewrite (IHn (fun v : Var => f1 (S v)) (fun v : Var => f2 (S v))).
+    rewrite H. show_dimensions. repeat rewrite dim_eq_lemma_2. reflexivity.
+    intros. rewrite H. reflexivity.
+Qed.
+Lemma ctx_to_matrix_eq_1 : forall n f1 f2,
+    (forall x, f1 x = f2 x) ->
+    ctx_to_matrix (list_of_Qubits n) f1 = ctx_to_matrix (list_of_Qubits n) f2.
+Proof.
+  induction n.
+  - intros. matrix_denote. solve_matrix.
+  - intros.
+    specialize (IHn (fun v : Var => f1 (S v)) (fun v : Var => f2 (S v))).
+    unfold ctx_to_matrix in *.
+    unfold big_kron in *. simpl in *.
+    show_dimensions.
+    rewrite dim_eq_lemma_2.
+    rewrite dim_eq_lemma_2.
+    apply kron_eq_1.
+    + rewrite H. reflexivity.
+    + apply IHn. intros. apply H.
+Qed.
+
+Lemma carrier_circ_1_spec : forall (cin x y sum cout : bool),
+  ⟦carrier_circ_1⟧ (bools_to_matrix [cout; sum; y; x; cin])
+  = (bools_to_matrix [cout ⊕ (calc_cout cin x y); sum ; y; x; cin]).
+Proof.
+  intros.
+  unfold carrier_circ_1.
+  apply adder_cout_circ_spec.
+Qed.
+
+Lemma adder_circ_1_spec : forall (cin x y sum cout : bool),
+  ⟦adder_circ_1⟧ (bools_to_matrix [cout; sum; y; x; cin])
+  = (bools_to_matrix [cout ⊕ (calc_cout cin x y); sum ⊕ (calc_sum cin x y); y; x; cin]).
 Proof.
   intros.
   unfold adder_circ_1.
   rewrite inSeq_correct.
   - unfold compose_super.
     unfold denote. unfold Denote_Box.
-    unfold ctx_to_matrix. simpl.
+    unfold bools_to_matrix. simpl.
     rewrite_inPar.
-    + remember adder_z_circ_spec as H; clear HeqH.
+    + remember adder_sum_circ_spec as H; clear HeqH.
       unfold bools_to_matrix in H. simpl in H.
       rewrite H. clear H.
       simpl_rewrite id_circ_Id.
@@ -355,13 +461,63 @@ Proof.
   - apply adder_cout_circ_WT.
   - apply inPar_WT.
     + apply id_circ_WT.
-    + apply adder_z_circ_WT.
+    + apply adder_sum_circ_WT.
+Qed.
+(*
+Lemma adder_circ_1_spec : forall (cin x y sum cout : bool),
+  ⟦adder_circ_1⟧ (ctx_to_matrix (list_of_Qubits 5) (fun_of_bools [cout; sum; y; x; cin]))
+  = (ctx_to_matrix 
+      (list_of_Qubits 5) 
+      (fun_of_bools [cout ⊕ ⌈ adder_cout_bexp | fun_of_bools [sum; y; x; cin] ⌉; 
+                         sum ⊕ ⌈ adder_sum_bexp | fun_of_bools [y; x; cin] ⌉; y; x; cin])).
+Proof.
+  intros.
+  unfold adder_circ_1.
+  rewrite inSeq_correct.
+  - unfold compose_super.
+    unfold denote. unfold Denote_Box.
+    unfold ctx_to_matrix. simpl.
+    rewrite_inPar.
+    + remember adder_sum_circ_spec as H; clear HeqH.
+      unfold bools_to_matrix in H. simpl in H.
+      rewrite H. clear H.
+      simpl_rewrite id_circ_Id.
+      * remember adder_cout_circ_spec as H; clear HeqH.
+      unfold bools_to_matrix in H. simpl in H.
+        rewrite H. clear H.
+        reflexivity.
+      * apply WF_bool_to_matrix.
+  - apply adder_cout_circ_WT.
+  - apply inPar_WT.
+    + apply id_circ_WT.
+    + apply adder_sum_circ_WT.
+Qed.
+*)
+Lemma carrier_circ_1_with_pads_spec : forall (n : nat) (f : Var -> bool),
+⟦carrier_circ_1_with_pads n⟧ (ctx_to_matrix (list_of_Qubits (5+n)) f)
+= (bool_to_matrix ((f 0) ⊕ ⌈ adder_cout_bexp | (fun x => f (S x)) ⌉)) ⊗
+  ((bool_to_matrix (f 1)) ⊗ (ctx_to_matrix (list_of_Qubits (3+n)) (fun x => f (S (S x))))).
+Proof.
+  intros.
+  unfold carrier_circ_1_with_pads.
+  Opaque denote. simpl_eq. Transparent denote.
+  assert (H1 : forall n f, length (ctx_to_mat_list (list_of_Qubits n) f) = 
+                           size_ctx (list_of_Qubits n)).
+  { induction n0.
+    - easy.
+    - intros. simpl. rewrite IHn0. easy. }
+  remember adder_cout_circ_with_pads_spec as H; clear HeqH.
+  specialize (H n%nat (fun (x : Var) => f x)).
+  unfold ctx_to_matrix in *. simpl in *.
+  show_dimensions.
+  rewrite H1 in *. unfold list_of_Qubits in *.
+  rewrite H. reflexivity.
 Qed.
 
 Lemma adder_circ_1_with_pads_spec : forall (n : nat) (f : Var -> bool),
 ⟦adder_circ_1_with_pads n⟧ (ctx_to_matrix (list_of_Qubits (5+n)) f)
 = (bool_to_matrix ((f 0) ⊕ ⌈ adder_cout_bexp | (fun x => f (S x)) ⌉)) ⊗
-  ((bool_to_matrix ((f 1) ⊕ ⌈ adder_z_bexp | (fun x => f (S (S x))) ⌉)) ⊗
+  ((bool_to_matrix ((f 1) ⊕ ⌈ adder_sum_bexp | (fun x => f (S (S x))) ⌉)) ⊗
   (ctx_to_matrix (list_of_Qubits (3+n)) (fun x => f (S (S x))))).
 Proof.
   intros.
@@ -378,7 +534,7 @@ Proof.
       { induction n0.
         - easy.
         - intros. simpl. rewrite IHn0. easy. }
-      remember adder_z_circ_with_pads_spec as H; clear HeqH.
+      remember adder_sum_circ_with_pads_spec as H; clear HeqH.
       specialize (H n%nat (fun (x : Var) => f (S x))).
       unfold ctx_to_matrix in H.
       simpl in *. unfold kron at 5.
@@ -406,7 +562,7 @@ Proof.
   - apply adder_cout_circ_with_pads_WT.
   - apply inPar_WT.
     + apply id_circ_WT.
-    + apply adder_z_circ_with_pads_WT.
+    + apply adder_sum_circ_with_pads_WT.
 Qed.
 Close Scope matrix_scope.
 
@@ -444,11 +600,1129 @@ Lemma adder_circ_1_test_111 :
 Proof. apply adder_circ_1_spec. Qed.
 
 (*
-Input : (cout, (z1, (y1, (x1, (z2, (y2, (x2, ... , (zn, (yn, (xn, (cin, ())))))))))))
-Output : (cout', (z1', (y1, (x1, (z2', (y2, (x2, ... , (zn', (yn, (xn, (cin, ())))))))))))
+Input : (cout, (sum1, (y1, (x1, (sum2, (y2, (x2, ... , (sumn, (yn, (xn, (cin, ())))))))))))
+Output : (cout', (sum1', (y1, (x1, (sum2', (y2, (x2, ... , (sumn', (yn, (xn, (cin, ())))))))))))
 *)
 
+Open Scope nat_scope.
+
 (* This can be refactored using init_at *)
+Program Fixpoint adder_circ_n_left (n : nat) : Box ((1+3*n) ⨂ Qubit) ((1+4*n) ⨂ Qubit) := 
+  match n with
+  | O => id_circ
+  | S n' => (@id_circ Qubit ∥ (@id_circ Qubit ∥ (@id_circ Qubit ∥ (adder_circ_n_left n')))) ;;
+            (init_at false (4*n) 0) ;;
+            (adder_circ_1_with_pads (4*n'))
+  end.
+Next Obligation.
+  replace (S n' + (S n' + (S n' + (S n' + 0))))
+    with (4 + n' + (n' + (n' + (n' + 0)))) by omega.
+  simpl. reflexivity.
+Defined.
+Next Obligation.
+  replace (S n' + (S n' + (S n' + (S n' + 0))))
+    with (4 + n' + (n' + (n' + (n' + 0)))) by omega.
+  simpl. reflexivity.
+Defined.
+Next Obligation.
+  replace (n' + S (n' + S (n' + 0))) with (2 + n' + (n' + (n' + 0))) by omega.
+  simpl. reflexivity.
+Defined.
+Next Obligation.
+  replace (n' + S (n' + S (n' + S (n' + 0))))
+    with (3 + (n' + (n' + (n' + (n' + 0))))) by omega.
+  simpl. reflexivity.
+Defined.
+Program Fixpoint adder_circ_n_right (n : nat) : Box ((1+4*n) ⨂ Qubit) ((1+3*n) ⨂ Qubit) := 
+  match n with
+  | O => id_circ
+  | S n' => (carrier_circ_1_with_pads (4*n')) ;;
+            (assert_at false (4*n) 0) ;;
+            (@id_circ Qubit ∥ (@id_circ Qubit ∥ (@id_circ Qubit ∥ (adder_circ_n_right n')))) 
+  end.
+Next Obligation.
+  replace (S n' + (S n' + (S n' + (S n' + 0))))
+    with (4 + (n' + (n' + (n' + (n' + 0))))) by omega.
+  simpl. reflexivity.
+Defined.
+Next Obligation.
+  replace (S n' + (S n' + (S n' + (S n' + 0))))
+    with (4 + (n' + (n' + (n' + (n' + 0))))) by omega.
+  simpl. reflexivity.
+Defined.
+Next Obligation.
+  replace (n' + S (n' + S (n' + S (n' + 0))))
+    with (3 + (n' + (n' + (n' + (n' + 0))))) by omega.
+  simpl. reflexivity.
+Defined.
+Next Obligation.
+  replace (n' + S (n' + S (n' + 0))) with (2 + n' + (n' + (n' + 0))) by omega.
+  simpl. reflexivity.
+Defined.
+Program Fixpoint adder_circ_n (n : nat) : Box ((2+3*n) ⨂ Qubit) ((2+3*n) ⨂ Qubit) := 
+  match n with
+  | O => calc_id_circ
+  | S n' => (id_circ ∥ (id_circ ∥ (id_circ ∥ (id_circ ∥ (adder_circ_n_left n'))))) ;; 
+            (adder_circ_1_with_pads (4*n')) ;;
+            (id_circ ∥ (id_circ ∥ (id_circ ∥ (id_circ ∥ (adder_circ_n_right n')))))
+  end.
+Next Obligation.
+  replace (n' + S (n' + S (n' + 0)))
+    with (2 + (n' + (n' + (n' + 0)))) by omega.
+  simpl. reflexivity.
+Defined.
+Next Obligation.
+  replace (n' + S (n' + S (n' + 0)))
+    with (2 + (n' + (n' + (n' + 0)))) by omega.
+  simpl. reflexivity.
+Defined.
+
+Lemma adder_circ_n_left_WT : forall (n : nat),
+    Typed_Box (adder_circ_n_left n).
+Proof.
+  induction n.
+  - unfold adder_circ_n_left. apply id_circ_WT.
+  - unfold adder_circ_n_left. simpl_eq.
+    apply inSeq_WT.
+    + compile_typing True. unfold adder_circ_n_left in IHn.
+      program_simpl.
+    + simpl_eq. apply inSeq_WT.
+      * apply strip_one_l_in_WT. apply inPar_WT.
+        { apply boxed_gate_WT. }
+        { simple_typing (inParMany_WT). }
+      * simpl_eq. apply adder_circ_1_with_pads_WT.
+Qed.
+Lemma adder_circ_n_right_WT : forall (n : nat),
+  Typed_Box (adder_circ_n_right n).
+Proof.
+  induction n.
+  - unfold adder_circ_n_right. apply id_circ_WT.
+  - unfold adder_circ_n_right. simpl_eq.
+    apply inSeq_WT.
+    + simpl_eq. apply carrier_circ_1_with_pads_WT.
+    + simpl_eq. apply inSeq_WT.
+      * apply strip_one_l_out_WT. apply inPar_WT.
+        { apply boxed_gate_WT. }
+        { simple_typing (inParMany_WT). }
+      * simpl_eq. compile_typing True. unfold adder_circ_n_right in IHn.
+        program_simpl.
+Qed.
+Lemma adder_circ_n_WT : forall (n : nat),
+  Typed_Box (adder_circ_n n).
+Proof.
+  induction n.
+  - unfold adder_circ_n. apply calc_id_circ_WT.
+  - unfold adder_circ_n. simpl_eq.
+    apply inSeq_WT.
+    + simple_typing (adder_circ_n_left_WT).
+    + apply inSeq_WT.
+      { apply adder_circ_1_with_pads_WT. }
+      { simple_typing (adder_circ_n_right_WT). }
+Qed.
+
+Open Scope matrix_scope.
+
+(* For n-adder specification *)
+
+Lemma mixed_state_big_kron_ctx_to_mat_list : forall n f,  Mixed_State (⨂ ctx_to_mat_list (list_of_Qubits n) f).
+Proof.
+  induction n.
+  - intros. simpl. show_mixed.
+  - intros. simpl.
+    specialize (mixed_kron 2) as H. apply H.
+    + show_mixed.
+    + apply IHn.
+Qed.
+
+Fixpoint n_adder_cout_bexp (n m : nat) : bexp :=
+  match m with
+  | O => b_var (1+n+n+n)%nat (* cin = b_var (1+n+n+n)%nat *)
+  | S m' => let i := (n-m)%nat in
+            b_xor (b_and (n_adder_cout_bexp n m') (b_xor (b_var (3+i+i+i)%nat) (b_var (2+i+i+i)%nat))) (b_and (b_var (3+i+i+i)%nat) (b_var (2+i+i+i)%nat))
+             (* cin = n_adder_cout_bexp n m'
+                x = b_var (3+i+i+i)%nat
+                y = b_var (2+i+i+i)%nat *)
+  end.
+
+Eval simpl in n_adder_cout_bexp 3 3.
+Eval simpl in n_adder_cout_bexp 3 2.
+Eval simpl in n_adder_cout_bexp 3 1.
+Eval simpl in n_adder_cout_bexp 3 0.
+
+Definition n_adder_sum_bexp (n m : nat) : bexp :=
+  match m with
+  | 0 => b_var (1+n+n+n)%nat (* cin = b_var (1+n+n+n)%nat *)
+  | S m' => let i := (n-m)%nat in
+            b_xor (n_adder_cout_bexp n m') (b_xor (b_var (3+i+i+i)%nat) (b_var (2+i+i+i)%nat))
+             (* cin = n_adder_cout_bexp n m'
+                x = b_var (3+i+i+i)%nat
+                y = b_var (2+i+i+i)%nat *)
+  end.
+
+Eval simpl in n_adder_sum_bexp 3 3.
+Eval simpl in n_adder_sum_bexp 3 2.
+Eval simpl in n_adder_sum_bexp 3 1.
+Eval simpl in n_adder_sum_bexp 3 0.
+
+Fixpoint increase_vars_by (k : nat) (b : bexp) : bexp :=
+  match b with
+  | b_t   => b_t
+  | b_f   => b_f
+  | b_var x => b_var (k + x)%nat
+  | b_not b' => b_not (increase_vars_by k b')
+  | b_and b1 b2 => b_and (increase_vars_by k b1) (increase_vars_by k b2)
+  | b_xor b1 b2 => b_xor (increase_vars_by k b1) (increase_vars_by k b2)
+  end.
+
+Lemma bexp_interpret_equiv_1 : forall (k : nat) (b : bexp) (f : Var -> bool),
+    ⌈ b | fun x : Var => f (k + x)%nat ⌉
+    = ⌈ increase_vars_by k b | f ⌉.
+Proof.
+  induction b.
+  - intros. simpl. reflexivity.
+  - intros. simpl. reflexivity.
+  - intros. simpl. reflexivity.
+  - intros. simpl. rewrite IHb. reflexivity.
+  - intros. simpl. rewrite IHb1. rewrite IHb2. reflexivity.
+  - intros. simpl. rewrite IHb1. rewrite IHb2. reflexivity.
+Qed.
+
+Lemma n_adder_cout_bexp_equiv_1 : forall (n m : nat),
+    (m <= n)%nat ->
+    increase_vars_by 3%nat (n_adder_cout_bexp n m) = n_adder_cout_bexp (S n) m.
+Proof.
+  intros. generalize dependent n.
+  induction m.
+  - intros. simpl. replace (n + S n + S n)%nat with (2 + n + n + n)%nat by omega.
+    reflexivity.
+  - intros. simpl. rewrite IHm.
+    remember (n - S m)%nat as i.
+    replace (n - m)%nat with (1 + i)%nat by omega. simpl.
+    replace (i + S i + S i)%nat with (2 + i + i + i)%nat by omega. simpl.
+    reflexivity.
+    omega.
+Qed.
+
+Lemma n_adder_sum_bexp_equiv_1 : forall (n m : nat),
+    (m <= n)%nat ->
+    increase_vars_by 3%nat (n_adder_sum_bexp n m) = n_adder_sum_bexp (S n) m.
+Proof.
+  intros. generalize dependent n.
+  induction m.
+  - intros. simpl. replace (n + S n + S n)%nat with (2 + n + n + n)%nat by omega.
+    reflexivity.
+  - intros. simpl. rewrite n_adder_cout_bexp_equiv_1.
+    remember (n - S m)%nat as i.
+    replace (n - m)%nat with (1 + i)%nat by omega. simpl.
+    replace (i + S i + S i)%nat with (2 + i + i + i)%nat by omega. simpl.
+    reflexivity.
+    omega.
+Qed.
+
+(* compute_adder_n_left
+   : Functional meaning of [adder_circ_n_left]
+     Input  (list of bools of length 3n+1) : [z0 y0 x0 z1 y1 x1 ... zn yn xn cin]
+     Output (list of bools of length 4n+1) : [c0 z0 y0 x0 c1 z1 y1 x1 ... cn zn yn xn cin]
+*)
+Fixpoint compute_adder_n_left (n : nat) (f : Var -> bool) : Var -> bool :=
+  match n with
+  | 0 => f
+  | S n' =>
+    (fun x => match x with
+              | 0 => ⌈ n_adder_cout_bexp n n |
+              (fun i => match i with
+                        | 0 => false
+                        | S i' => f i'
+                        end) ⌉
+              | 1 => (f 0) ⊕ ⌈ n_adder_sum_bexp n n |
+              (fun i => match i with
+                        | 0 => false
+                        | S i' => f i'
+                        end) ⌉
+              | 2 => f 1
+              | 3 => f 2
+              | S (S (S (S x'))) => (compute_adder_n_left n' (fun i => f (3 + i))) x'
+              end)
+  end.
+
+Definition compute_adder_n_left_inp_1 := (fun (x : Var) =>
+                     match x with
+                     | 0 => false
+                     | 1 => true
+                     | 2 => true
+                     | 3 => true
+                     | _ => false
+                     end).
+Eval compute in compute_adder_n_left 1 compute_adder_n_left_inp_1.
+
+Lemma adder_circ_n_spec_left_1 : forall (n : nat) (f : Var -> bool),
+    let l1 := list_of_Qubits (1 + 3 * n) in
+    let l2 := list_of_Qubits (1 + 4 * n) in
+    ⟦adder_circ_n_left n⟧ (ctx_to_matrix l1 f)
+    = (ctx_to_matrix l2 (compute_adder_n_left n f)).
+Proof.
+(*
+  Set Printing Implicit.
+*)
+  induction n.
+  - intros. unfold ctx_to_matrix. simpl.
+    remember id_circ_Id. simpl in *. apply e.
+    rewrite kron_1_r. apply WF_bool_to_matrix.
+  - intros. unfold list_of_Qubits in *.
+    Opaque compute_adder_n_left.
+    unfold adder_circ_n_left. unfold adder_circ_n_left in IHn.
+    Set Printing Implicit. show_dimensions. simpl_eq.
+    specialize inSeq_correct as IS. simpl in IS. rewrite IS. clear IS.
+    + unfold compose_super.
+      simpl_eq. program_simpl.
+      replace (n + S (n + S (n + S (n + 0)))) with (3 + (n + (n + (n + (n + 0))))) by omega.
+      specialize inSeq_correct as IS. simpl in IS. rewrite IS. clear IS.
+      * unfold compose_super. simpl_eq. program_simpl.
+        replace (ctx_to_matrix l1 f) with (bool_to_matrix (f 0) ⊗ ctx_to_matrix (list_of_Qubits (3 + 3*n)) (fun x => f (S x))).
+        { simpl. Set Printing All.
+          rewrite dim_eq_lemma_1.
+          specialize (inPar_correct
+                        Qubit Qubit
+                        (Tensor Qubit (Tensor Qubit (Tensor Qubit (NTensor (n + (n + (n + 0))) Qubit))))
+                        (Tensor Qubit (Tensor Qubit (Tensor Qubit (NTensor (n + (n + (n + (n + 0)))) Qubit)))))
+            as IP.
+          simpl in IP. rewrite dim_eq_lemma_3 in IP.
+          unfold list_of_Qubits. unfold ctx_to_matrix. simpl.
+          rewrite dim_eq_lemma_2. rewrite dim_eq_lemma_1. rewrite IP. clear IP.
+          - specialize (inPar_correct
+                          Qubit Qubit
+                          (Tensor Qubit (Tensor Qubit (NTensor (n + (n + (n + 0))) Qubit)))
+                          (Tensor Qubit (Tensor Qubit (NTensor (n + (n + (n + (n + 0)))) Qubit))))
+              as IP.
+            simpl in IP. rewrite dim_eq_lemma_3 in IP.
+            rewrite dim_eq_lemma_2. rewrite IP. clear IP.
+            + specialize (inPar_correct
+                            Qubit Qubit
+                            (Tensor Qubit (NTensor (n + (n + (n + 0))) Qubit))
+                            (Tensor Qubit (NTensor (n + (n + (n + (n + 0)))) Qubit)))
+                as IP.
+              simpl in IP. rewrite dim_eq_lemma_3 in IP.
+              rewrite IP. clear IP.
+              * replace (@kron
+                           (S (S O)) (S (S O))
+                           (Nat.pow (S (S O))
+                                    (Init.Nat.add n (Init.Nat.add n (Init.Nat.add n O))))
+                           (Nat.pow (S (S O))
+                                    (Init.Nat.add n (Init.Nat.add n (Init.Nat.add n O))))
+                           (bool_to_matrix (f 3))
+                           (big_kron (ctx_to_mat_list (repeat (Some Qubit) (n + (n + (n + 0)))) (fun v : Var => f (S (S (S (S v)))))))) with
+                    (ctx_to_matrix (repeat (Some Qubit) (1 + 3 * n)) (fun v : Var => f (S (S (S v))))).
+                { simpl in *. rewrite IHn. clear IHn.
+                  Unset Printing All. Unset Printing Implicit.
+                  specialize id_circ_Id as Iid. simpl in Iid. repeat rewrite Iid. clear Iid.
+                  Locate "⊗".
+                  - rewrite strip_one_l_in_eq.
+                    specialize (kron_1_l
+                                  (2 * (2 * (2 * 2 ^ ⟦ Some Qubit :: repeat (Some Qubit) (n + (n + (n + (n + 0)))) ⟧)))
+                                  (2 * (2 * (2 * 2 ^ ⟦ Some Qubit :: repeat (Some Qubit) (n + (n + (n + (n + 0)))) ⟧)))
+                                  (bool_to_matrix (f 0) ⊗ (bool_to_matrix (f 1) ⊗ (bool_to_matrix (f 2) ⊗ ctx_to_matrix (Some Qubit :: repeat (Some Qubit) (n + (n + (n + (n + 0))))) (compute_adder_n_left n (fun v : Var => f (S (S (S v))))))))) as IK.
+                    simpl in IK.
+                    Set Printing All. rewrite dim_eq_lemma_1 in IK. rewrite dim_eq_lemma_3.
+                    rewrite <- IK. Unset Printing All. clear IK.
+                    + Set Printing Implicit. Check inPar_correct.
+                      replace (n + S (n + S (n + S (n + 0)))) with (3 + (n + (n + (n + (n + 0))))) by omega.
+                      simpl.
+                      specialize (inPar_correct
+                                    One Qubit
+                                    (Tensor Qubit (NTensor (3 + (n + (n + (n + (n + 0))))) Qubit))
+                                    (Tensor Qubit (NTensor (3 + (n + (n + (n + (n + 0))))) Qubit))
+                                    init0 id_circ)
+                        as IP.
+                      simpl in IP. rewrite dim_eq_lemma_3 in IP.
+                      rewrite dim_eq_lemma_2. rewrite IP. clear IP.
+                      Unset Printing Implicit.
+                      * specialize init0_spec as IG. simpl in IG. rewrite IG. clear IG.
+                        specialize id_circ_Id as Iid. simpl in Iid. rewrite Iid. clear Iid.
+                        { Check adder_circ_1_with_pads_spec.
+                          Set Printing Implicit.
+                          specialize (adder_circ_1_with_pads_spec
+                                        (n + (n + (n + (n + 0))))
+                                        (fun x => match x with
+                                                  | 0 => false
+                                                  | 1 => f 0
+                                                  | 2 => f 1
+                                                  | 3 => f 2
+                                                  | S (S (S (S x'))) => (compute_adder_n_left n (fun v : Var => f (S (S (S v))))) x'
+                                                  end))
+                            as IA. unfold ctx_to_matrix in IA. simpl in IA.
+                          unfold ctx_to_matrix. simpl. Set Printing All.
+                          unfold NTensor in IA. unfold NTensor.
+                          rewrite dim_eq_lemma_1 in IA. rewrite dim_eq_lemma_2 in IA.
+                          rewrite dim_eq_lemma_2. rewrite IA. clear IA. Unset Printing All.
+                          repeat apply kron_eq_1.
+                          - clear l1. clear l2.
+                            Transparent compute_adder_n_left. simpl.
+                            replace (n - n + (n - n) + (n - n)) with 0 by omega.
+                            rewrite <- n_adder_cout_bexp_equiv_1; try apply Nat.le_refl.
+                            rewrite <- bexp_interpret_equiv_1.
+                            destruct n.
+                            + simpl. remember ((f 3 && f 2 ⊕ f 1) ⊕ (f 2 && f 1)).
+                              destruct b; reflexivity.
+                            + simpl.
+                              replace (n - n + (n - n) + (n - n)) with 0 by omega.
+                              rewrite <- n_adder_cout_bexp_equiv_1; try apply Nat.le_refl.
+                              rewrite <- bexp_interpret_equiv_1.
+                              rewrite <- bexp_interpret_equiv_1.
+                              simpl.
+                              remember (((⌈ n_adder_cout_bexp n n |
+                                          fun x : Var => f (S (S (S (S (S x))))) ⌉
+                                                           && f 5 ⊕ f 4)
+                                           ⊕ (f 5 && f 4) && f 2 ⊕ f 1) ⊕ (f 2 && f 1)).
+                              destruct b; reflexivity.
+                          - clear l1. clear l2.
+                            Transparent compute_adder_n_left. simpl.
+                            replace (n - n + (n - n) + (n - n)) with 0 by omega.
+                            rewrite <- n_adder_cout_bexp_equiv_1; try apply Nat.le_refl.
+                            rewrite <- bexp_interpret_equiv_1.
+                            destruct n.
+                            + simpl. reflexivity.
+                            + simpl. replace (n - n + (n - n) + (n - n)) with 0 by omega.
+                              rewrite <- n_adder_cout_bexp_equiv_1; try apply Nat.le_refl.
+                              rewrite <- bexp_interpret_equiv_1.
+                              rewrite <- bexp_interpret_equiv_1.
+                              simpl. reflexivity.
+                          - simpl. reflexivity.
+                          - simpl. reflexivity.
+                          - simpl. reflexivity.
+                          - simpl. reflexivity.
+                        }
+                        clear l1. clear l2.
+                        apply WF_kron; simpl; try rewrite dim_eq_lemma_3; try reflexivity; try apply WF_bool_to_matrix.
+                        apply WF_kron; simpl; try rewrite dim_eq_lemma_3; try reflexivity; try apply WF_bool_to_matrix.
+                        apply WF_kron; simpl; try rewrite dim_eq_lemma_3; try reflexivity; try apply WF_bool_to_matrix.
+                        specialize (WF_ctx_to_matrix (@Some WType Qubit :: @repeat (option WType) (@Some WType Qubit) (n + (n + (n + (n + 0)))))) as IW. simpl in IW. rewrite dim_eq_lemma_1 in IW. apply IW.
+                      * apply (init_WT false).
+                      * apply id_circ_WT.
+                      * show_mixed.
+                      * unfold ctx_to_matrix.
+                        repeat (try apply (mixed_kron 2); try apply mixed_big_kron; try show_mixed).
+                        specialize (mixed_state_big_kron_ctx_to_mat_list (1 + n + (n + (n + (n + 0)))) (compute_adder_n_left n (fun v : Var => f (S (S (S v))))))
+                          as Hmixed. rewrite dim_eq_lemma_2 in Hmixed. simpl in Hmixed. apply Hmixed.
+                    + apply WF_kron; simpl; try rewrite dim_eq_lemma_3; try reflexivity; try apply WF_bool_to_matrix.
+                      apply WF_kron; simpl; try rewrite dim_eq_lemma_3; try reflexivity; try apply WF_bool_to_matrix.
+                      apply WF_kron; simpl; try rewrite dim_eq_lemma_3; try reflexivity; try apply WF_bool_to_matrix.
+                      specialize (WF_ctx_to_matrix (@Some WType Qubit :: @repeat (option WType) (@Some WType Qubit) (n + (n + (n + (n + 0)))))) as IW. simpl in IW. rewrite dim_eq_lemma_1 in IW. apply IW.
+                  - apply WF_bool_to_matrix.
+                  - apply WF_bool_to_matrix.
+                  - apply WF_bool_to_matrix.
+                }
+                { unfold ctx_to_matrix. simpl. rewrite dim_eq_lemma_2. reflexivity. }
+              * apply id_circ_WT.
+              * apply adder_circ_n_left_WT.
+              * show_mixed.
+              * repeat (try apply (mixed_kron 2); try apply mixed_big_kron; try show_mixed).
+                specialize (mixed_state_big_kron_ctx_to_mat_list (n + (n + (n + 0))) (fun v : Var => f (S (S (S (S v))))))
+                  as Hmixed. rewrite dim_eq_lemma_2 in Hmixed. simpl in Hmixed. apply Hmixed.
+            + apply id_circ_WT.
+            + repeat apply inPar_WT; try apply id_circ_WT; try apply adder_circ_n_left_WT.
+            + show_mixed.
+            + repeat (try apply (mixed_kron 2); try apply mixed_big_kron; try show_mixed).
+              specialize (mixed_state_big_kron_ctx_to_mat_list (n + (n + (n + 0))) (fun v : Var => f (S (S (S (S v))))))
+                as Hmixed. rewrite dim_eq_lemma_2 in Hmixed. simpl in Hmixed. apply Hmixed.
+          - apply id_circ_WT.
+          - repeat apply inPar_WT; try apply id_circ_WT; try apply adder_circ_n_left_WT.
+          - show_mixed.
+          - repeat (try apply (mixed_kron 2); try apply mixed_big_kron; try show_mixed).
+            specialize (mixed_state_big_kron_ctx_to_mat_list (n + (n + (n + 0))) (fun v : Var => f (S (S (S (S v))))))
+              as Hmixed. rewrite dim_eq_lemma_2 in Hmixed. simpl in Hmixed. apply Hmixed.
+        }
+        { unfold ctx_to_matrix. simpl.
+          replace (n + S (n + S (n + 0))) with (2 + (n + (n + (n + 0)))) by omega.
+          simpl. rewrite dim_eq_lemma_2. rewrite dim_eq_lemma_1. reflexivity. }
+      * simpl_eq. apply adder_circ_1_with_pads_WT.
+      * apply strip_one_l_in_WT. apply inPar_WT; [apply (init_WT false) | apply id_circ_WT].
+    + simpl_eq. apply inSeq_WT.
+      * apply strip_one_l_in_WT. apply inPar_WT; [apply (init_WT false) | apply id_circ_WT].
+      * simpl_eq. apply adder_circ_1_with_pads_WT.
+    + repeat (apply inPar_WT; try apply id_circ_WT). apply adder_circ_n_left_WT.
+Qed.
+
+(* compute_adder_n_right
+   : Functional meaning of [adder_circ_n_right]
+     Input  (list of bools of length 4n+1) : [c0 z0 y0 x0 c1 z1 y1 x1 ... cn zn yn xn cin]
+     Output (list of bools of length 3n+1) : [z0 y0 x0 z1 y1 x1 ... zn yn xn cin]
+*)
+Fixpoint compute_adder_n_right (n : nat) (f : Var -> bool) : Var -> bool :=
+  match n with
+  | 0 => f
+  | S n' =>
+    (fun x => match x with
+              | 0 => f 1
+              | 1 => f 2
+              | 2 => f 3
+              | S (S (S x')) => (compute_adder_n_right n' (fun i => f (4 + i))) x'
+              end)
+  end.
+
+Definition compute_adder_n_right_inp_1 := (fun (x : Var) =>
+                     match x with
+                     | 0 => true
+                     | 1 => true
+                     | 2 => true
+                     | 3 => true
+                     | 4 => true
+                     | _ => false
+                     end).
+Eval compute in compute_adder_n_right 1 compute_adder_n_right_inp_1.
+
+Lemma adder_circ_n_spec_right_1 : forall (n : nat) (f : Var -> bool),
+    let l1 := list_of_Qubits (1 + 4 * n) in
+    let l2 := list_of_Qubits (1 + 3 * n) in
+    ⟦adder_circ_n_right n⟧
+      (ctx_to_matrix
+         l1
+         (fun x =>
+            match x with
+            | 0 => (compute_adder_n_left n (fun v : Var => f (S (S (S (S v))))) 0)
+            | S x' =>
+              (fun v : Var =>
+                 compute_adder_n_left n (fun v0 : Var => f (S (S (S (S v0))))) (S v)) x'
+            end))
+    = (ctx_to_matrix
+         l2 (compute_adder_n_right
+               n
+               (fun x =>
+                  match x with
+                  | 0 => (compute_adder_n_left n (fun v : Var => f (S (S (S (S v))))) 0)
+                  | S x' =>
+                    (fun v : Var =>
+                       compute_adder_n_left n (fun v0 : Var => f (S (S (S (S v0))))) (S v)) x'
+                  end))).
+Proof.
+  induction n.
+  - intros. simpl.
+    specialize id_circ_Id as Iid. simpl in Iid. repeat rewrite Iid. clear Iid. reflexivity.
+    apply WF_kron; try reflexivity; try apply WF_bool_to_matrix; try apply WF_Id.
+  - intros. simpl_eq.
+    replace (n - n + (n - n) + (n - n)) with 0 in * by omega.
+    specialize inSeq_correct as IS. simpl in IS. rewrite IS. clear IS.
+    + unfold compose_super. simpl_eq.
+      specialize inSeq_correct as IS. simpl in IS. rewrite IS. clear IS.
+      * unfold compose_super. simpl_eq.
+        specialize (carrier_circ_1_with_pads_spec
+                      (n + (n + (n + (n + 0))))
+                      (fun x => match x with
+                                | 0 => ((⌈ n_adder_cout_bexp (S n) n
+                                        | fun i : Var => match i with
+                                                         | 0 => false
+                                                         | S i' => f (S (S (S (S i'))))
+                                                         end ⌉ && f 6 ⊕ f 5) ⊕ (f 6 && f 5))
+                                | 1 => (f 4
+                                          ⊕ (⌈ n_adder_cout_bexp (S n) n
+                                            | fun i : Var =>
+                                                match i with
+                                                | 0 => false
+                                                | S i' => f (S (S (S (S i'))))
+                                                end ⌉ ⊕ (f 6 ⊕ f 5)))
+                                | S (S x') => (fun v : Var =>
+                                                 match v with
+                                                 | 0 => f 5
+                                                 | 1 => f 6
+                                                 | S (S v') =>
+                                                   compute_adder_n_left n
+                                                                        (fun i : Var => f (S (S (S (S (S (S (S i)))))))) v'
+                                                 end) x'
+                                end)) as H.
+        unfold ctx_to_matrix in *. simpl in *.
+        replace (n + S (n + S (n + S (n + 0)))) with (3 + n + (n + (n + (n + 0)))) by omega.
+        simpl. rewrite dim_eq_lemma_1 in *. rewrite dim_eq_lemma_2 in *.
+        rewrite H. clear H.
+
+        rewrite strip_one_l_out_eq.
+
+        specialize (inPar_correct
+                      Qubit One
+                      (NTensor (4 + n + (n + (n + (n + 0)))) Qubit)
+                      (NTensor (4 + n + (n + (n + (n + 0)))) Qubit))
+          as IP.
+        simpl in IP. rewrite dim_eq_lemma_3 in *. rewrite dim_eq_lemma_2 in *.
+        rewrite IP. clear IP.
+
+        { rewrite <- n_adder_cout_bexp_equiv_1; try apply Nat.le_refl.
+          rewrite <- bexp_interpret_equiv_1. simpl.
+          assert (H : ⌈ n_adder_cout_bexp n n |
+                  fun x : Var => f (S (S (S (S (S (S x)))))) ⌉
+                                 = compute_adder_n_left n (fun i : Var => f (S (S (S (S (S (S (S i)))))))) 0).
+          { destruct n.
+            - simpl. reflexivity.
+            - simpl. replace (n - n + (n - n) + (n - n)) with 0 by omega.
+              rewrite <- n_adder_cout_bexp_equiv_1; try apply Nat.le_refl.
+              rewrite <- bexp_interpret_equiv_1.
+              rewrite <- bexp_interpret_equiv_1.
+              simpl. reflexivity. }
+          rewrite H. clear H.
+          remember ((compute_adder_n_left n (fun i : Var => f (S (S (S (S (S (S (S i)))))))) 0 && f 6 ⊕ f 5) ⊕ (f 6 && f 5)).
+          rewrite xorb_nilpotent. clear b Heqb. simpl.
+          specialize assert0_spec as IA. simpl in IA. rewrite IA. clear IA.
+
+          rewrite kron_1_l.
+          - specialize id_circ_Id as Iid. simpl in Iid. repeat rewrite Iid. clear Iid.
+            + specialize (inPar_correct
+                            Qubit Qubit
+                            (NTensor (3 + n + (n + (n + (n + 0)))) Qubit)
+                            (NTensor (3 + n + (n + (n + 0))) Qubit))
+                as IP.
+              simpl in IP. rewrite dim_eq_lemma_3 in *.
+              rewrite IP. clear IP.
+              * specialize (inPar_correct
+                              Qubit Qubit
+                              (NTensor (2 + n + (n + (n + (n + 0)))) Qubit)
+                              (NTensor (2 + n + (n + (n + 0))) Qubit))
+                  as IP.
+                simpl in IP. rewrite dim_eq_lemma_3 in *.
+                rewrite IP. clear IP.
+                { specialize (inPar_correct
+                                Qubit Qubit
+                                (NTensor (1 + n + (n + (n + (n + 0)))) Qubit)
+                                (NTensor (1 + n + (n + (n + 0))) Qubit))
+                    as IP.
+                  simpl in IP. rewrite dim_eq_lemma_3 in *.
+                  rewrite IP. clear IP.
+                  - specialize id_circ_Id as Iid. simpl in Iid. repeat rewrite Iid. clear Iid.
+                    + replace (n + S (n + S (n + 0))) with (2 + n + (n + (n + 0))) by omega.
+                      simpl. rewrite dim_eq_lemma_3. repeat apply kron_eq_1.
+                      * reflexivity.
+                      * reflexivity.
+                      * rewrite dim_eq_lemma_2. apply kron_eq_1.
+                        { reflexivity. }
+                        { specialize (IHn (fun i : Var => f (S (S (S i))))) as H.
+                          simpl in H. rewrite dim_eq_lemma_2 in H. rewrite H.
+                          rewrite dim_eq_lemma_2. apply kron_eq_1.
+                          - destruct n.
+                            + simpl. reflexivity.
+                            + simpl. reflexivity.
+                          - destruct n.
+                            + simpl. reflexivity.
+                            + simpl. reflexivity. }
+                    + apply WF_bool_to_matrix.
+                    + apply WF_bool_to_matrix.
+                    + apply WF_bool_to_matrix.
+                  - apply id_circ_WT.
+                  - apply adder_circ_n_right_WT.
+                  - show_mixed.
+                  - repeat (try apply (mixed_kron 2); try apply mixed_big_kron; try show_mixed).
+                    specialize (mixed_state_big_kron_ctx_to_mat_list (n + (n + (n + (n + 0)))) (fun v : Var => compute_adder_n_left n (fun i : Var => f (S (S (S (S (S (S (S i)))))))) (S v)))
+                      as Hmixed. rewrite dim_eq_lemma_2 in Hmixed. simpl in Hmixed. apply Hmixed.
+                }
+                { apply id_circ_WT. }
+                { apply inPar_WT.
+                  - apply id_circ_WT.
+                  - apply adder_circ_n_right_WT. }
+                { show_mixed. }
+                { repeat (try apply (mixed_kron 2); try apply mixed_big_kron; try show_mixed).
+                  specialize (mixed_state_big_kron_ctx_to_mat_list (n + (n + (n + (n + 0)))) (fun v : Var => compute_adder_n_left n (fun i : Var => f (S (S (S (S (S (S (S i)))))))) (S v))) as Hmixed.
+                  rewrite dim_eq_lemma_2 in Hmixed. simpl in Hmixed. apply Hmixed. }
+              * apply id_circ_WT.
+              * repeat apply inPar_WT; try apply id_circ_WT. apply adder_circ_n_right_WT.
+              * show_mixed.
+              * repeat (try apply (mixed_kron 2); try apply mixed_big_kron; try show_mixed).
+                specialize (mixed_state_big_kron_ctx_to_mat_list (n + (n + (n + (n + 0)))) (fun v : Var => compute_adder_n_left n (fun i : Var => f (S (S (S (S (S (S (S i)))))))) (S v))) as Hmixed.
+                rewrite dim_eq_lemma_2 in Hmixed. simpl in Hmixed. apply Hmixed. 
+            + repeat apply WF_kron; try reflexivity; try apply WF_bool_to_matrix.
+              * simpl. rewrite dim_eq_lemma_3. reflexivity.
+              * simpl. rewrite dim_eq_lemma_3. reflexivity.
+              * specialize (WF_ctx_to_matrix (@repeat (option WType) (@Some WType Qubit) (n + (n + (n + (n + 0)))))) as IW. simpl in IW. rewrite dim_eq_lemma_1 in IW. apply IW.
+          - specialize id_circ_Id as Iid. simpl in Iid. repeat rewrite Iid. clear Iid.
+            repeat apply WF_kron; try reflexivity; try apply WF_bool_to_matrix.
+            specialize (WF_ctx_to_matrix (@repeat (option WType) (@Some WType Qubit) (n + (n + (n + (n + 0)))))) as IW. simpl in IW. rewrite dim_eq_lemma_1 in IW. apply IW.
+            simpl. rewrite dim_eq_lemma_3.
+            repeat apply WF_kron; try reflexivity; try apply WF_bool_to_matrix.
+            specialize (WF_ctx_to_matrix (@repeat (option WType) (@Some WType Qubit) (n + (n + (n + (n + 0)))))) as IW. simpl in IW. rewrite dim_eq_lemma_1 in IW. apply IW.
+        }
+        { apply (assert_WT false). }
+        { apply id_circ_WT. }
+        { show_mixed. }
+        { repeat (try apply (mixed_kron 2); try apply mixed_big_kron; try show_mixed).
+          specialize (mixed_state_big_kron_ctx_to_mat_list (n + (n + (n + (n + 0)))) (fun v : Var => compute_adder_n_left n (fun i : Var => f (S (S (S (S (S (S (S i)))))))) (S v))) as Hmixed.
+          rewrite dim_eq_lemma_2 in Hmixed. simpl in Hmixed. apply Hmixed. }
+      * simpl_eq. repeat (apply inPar_WT; try apply id_circ_WT).
+        apply adder_circ_n_right_WT.
+      * apply strip_one_l_out_WT.
+        apply inPar_WT; [apply (assert_WT false) | apply id_circ_WT].
+    + simpl_eq. apply inSeq_WT.
+      * apply strip_one_l_out_WT.
+        apply inPar_WT; [apply (assert_WT false) | apply id_circ_WT].
+      * simpl_eq. repeat (apply inPar_WT; try apply id_circ_WT).
+        apply adder_circ_n_right_WT.
+    + apply carrier_circ_1_with_pads_WT.
+Qed.
+
+(* compute_adder_n_aux
+   : Helper function for defining functional meaning of [adder_circ_n]
+     Input  (list of bools of length 3n+1) : [z0 y0 x0 z1 y1 x1 ... zn yn xn cin]
+     Output (list of bools of length 3n+1) : [z0 y0 x0 z1 y1 x1 ... zn yn xn cin]
+*)
+Fixpoint compute_adder_n_aux (n : nat) (f : Var -> bool) : Var -> bool :=
+  match n with
+  | 0 => f
+  | S n' =>
+    (fun x => match x with
+              | 0 => (f 0) ⊕ ⌈ n_adder_sum_bexp n n |
+              (fun i => match i with
+                        | 0 => false
+                        | S i' => f i'
+                        end) ⌉
+              | 1 => f 1
+              | 2 => f 2
+              | S (S (S x')) => (compute_adder_n_aux n' (fun i => f (3 + i))) x'
+              end)
+  end.
+(* compute_adder_n
+   : Functional meaning of [adder_circ_n]
+     Input  (list of bools of length 3n+2) : [cout z0 y0 x0 z1 y1 x1 ... zn yn xn cin]
+     Output (list of bools of length 3n+2) : [cout z0 y0 x0 z1 y1 x1 ... zn yn xn cin]
+ *)
+Fixpoint compute_adder_n (n : nat) (f : Var -> bool) : Var -> bool :=
+  match n with
+  | 0 => (fun x => match x with
+                   | 0 => (f 0) ⊕ (f 1)
+                   | _ => f x
+                   end)
+  | S n' => (fun x => match x with
+                      | 0 => (f 0) ⊕ ⌈ n_adder_cout_bexp n n |
+                      (fun i => match i with
+                                | 0 => false
+                                | S i' => f (S i')
+                                end) ⌉
+                      | S x' => (compute_adder_n_aux n (fun i => f (S i)) x')
+                      end)
+  end.
+
+Definition compute_adder_n_inp_1 := (fun (x : Var) =>
+                     match x with
+                     | 0 => false
+                     | 1 => false
+                     | 2 => true
+                     | 3 => true
+                     | 4 => true
+                     | _ => false
+                     end).
+Eval compute in compute_adder_n 1 compute_adder_n_inp_1.
+
+Lemma adder_circ_n_spec_1 : forall (n : nat) (f : Var -> bool),
+    let l1 := list_of_Qubits (2 + 3 * n) in
+    let l2 := list_of_Qubits (2 + 3 * n) in
+    ⟦adder_circ_n n⟧ (ctx_to_matrix l1 f)
+    = (ctx_to_matrix l2 (compute_adder_n n f)).
+Proof.
+(*
+  Set Printing Implicit.
+ *)
+  destruct n.
+  - intros. unfold ctx_to_matrix. simpl.
+    specialize (calc_id_circ_spec (f 1) (f 0)) as H.
+    unfold fun_of_bools in H. unfold bools_to_matrix in H.
+    simpl in *. rewrite H. reflexivity.
+  - intros. unfold list_of_Qubits in *.
+    Opaque compute_adder_n.
+    unfold adder_circ_n. simpl_eq.
+    unfold list_of_Qubits. unfold ctx_to_matrix. simpl.
+    replace (n + S (n + S (n + 0))) with (2 + n + (n + (n + 0))) by omega. simpl.
+    specialize inSeq_correct as IS. simpl in IS. rewrite IS. clear IS.
+    + unfold compose_super.
+      specialize inSeq_correct as IS. simpl in IS. rewrite IS. clear IS.
+      * unfold compose_super.
+        specialize (inPar_correct
+                      Qubit Qubit
+                      (NTensor (4 + n + (n + (n + 0))) Qubit)
+                      (NTensor (4 + n + (n + (n + (n + 0)))) Qubit))
+          as IP.
+        simpl in IP. rewrite dim_eq_lemma_3 in IP.
+        rewrite dim_eq_lemma_2. rewrite dim_eq_lemma_1. rewrite dim_eq_lemma_2.
+        rewrite dim_eq_lemma_3 in IP.
+        rewrite IP. clear IP.
+        { specialize (inPar_correct
+                        Qubit Qubit
+                        (NTensor (3 + n + (n + (n + 0))) Qubit)
+                        (NTensor (3 + n + (n + (n + (n + 0)))) Qubit))
+            as IP.
+          simpl in IP. rewrite dim_eq_lemma_3 in IP.
+          rewrite dim_eq_lemma_3 in IP.
+          rewrite IP. clear IP.
+          - specialize (inPar_correct
+                          Qubit Qubit
+                          (NTensor (2 + n + (n + (n + 0))) Qubit)
+                          (NTensor (2 + n + (n + (n + (n + 0)))) Qubit))
+              as IP.
+            simpl in IP. rewrite dim_eq_lemma_3 in IP.
+            rewrite dim_eq_lemma_3 in IP.
+            rewrite IP. clear IP.
+            + specialize (inPar_correct
+                            Qubit Qubit
+                            (NTensor (1 + n + (n + (n + 0))) Qubit)
+                            (NTensor (1 + n + (n + (n + (n + 0)))) Qubit))
+                as IP.
+              simpl in IP. rewrite dim_eq_lemma_3 in IP.
+              rewrite dim_eq_lemma_3 in IP.
+              rewrite IP. clear IP.
+              * specialize id_circ_Id as Iid. simpl in Iid. repeat rewrite Iid. clear Iid.
+                specialize
+                  (adder_circ_n_spec_left_1 n (fun v => f (4 + v))) as H.
+                simpl in H. unfold ctx_to_matrix in H. simpl in H.
+                rewrite dim_eq_lemma_1 in H. rewrite dim_eq_lemma_2 in H. rewrite H. clear H.
+                { simpl. rewrite dim_eq_lemma_2.
+                  specialize
+                    (adder_circ_1_with_pads_spec
+                       (n + (n + (n + (n + 0))))
+                       (fun x => match x with
+                                 | 0 => f 0
+                                 | 1 => f 1
+                                 | 2 => f 2
+                                 | 3 => f 3
+                                 | S (S (S (S x'))) => (compute_adder_n_left n (fun v : Var => f (S (S (S (S v))))) x')
+                                 end)) as H.
+                  simpl in H. unfold ctx_to_matrix in H. simpl in H.
+                  rewrite dim_eq_lemma_1 in H. rewrite dim_eq_lemma_2 in H.
+                  rewrite H. clear H.
+                  
+                  specialize (inPar_correct
+                                Qubit Qubit
+                                (NTensor (4 + n + (n + (n + (n + 0)))) Qubit)
+                                (NTensor (4 + n + (n + (n + 0))) Qubit))
+                    as IP.
+                  simpl in IP. rewrite dim_eq_lemma_3 in IP.
+                  rewrite dim_eq_lemma_3 in IP.
+                  rewrite IP. clear IP.
+                  - specialize (inPar_correct
+                                  Qubit Qubit
+                                  (NTensor (3 + n + (n + (n + (n + 0)))) Qubit)
+                                  (NTensor (3 + n + (n + (n + 0))) Qubit))
+                      as IP.
+                    simpl in IP. rewrite dim_eq_lemma_3 in IP.
+                    rewrite dim_eq_lemma_3 in IP.
+                    rewrite IP. clear IP.
+                    + specialize (inPar_correct
+                                    Qubit Qubit
+                                    (NTensor (2 + n + (n + (n + (n + 0)))) Qubit)
+                                    (NTensor (2 + n + (n + (n + 0))) Qubit))
+                        as IP.
+                      simpl in IP. rewrite dim_eq_lemma_3 in IP.
+                      rewrite dim_eq_lemma_3 in IP.
+                      rewrite IP. clear IP.
+                      * specialize (inPar_correct
+                                      Qubit Qubit
+                                      (NTensor (1 + n + (n + (n + (n + 0)))) Qubit)
+                                      (NTensor (1 + n + (n + (n + 0))) Qubit))
+                          as IP.
+                        simpl in IP. rewrite dim_eq_lemma_3 in IP.
+                        rewrite dim_eq_lemma_3 in IP.
+                        rewrite IP. clear IP.
+                        { specialize id_circ_Id as Iid. simpl in Iid. repeat rewrite Iid.
+                          clear Iid.
+                          - repeat apply kron_eq_1.
+                            + Transparent compute_adder_n. simpl.
+                              destruct n.
+                              * simpl. reflexivity.
+                              * simpl. replace (match n with
+                                                | 0 => S n
+                                                | S l => n - l
+                                                end) with 1.
+                                replace (n - n + (n - n) + (n - n)) with 0 in * by omega.
+                                rewrite <- n_adder_cout_bexp_equiv_1; try apply Nat.le_refl.
+                                rewrite <- n_adder_cout_bexp_equiv_1; try (apply le_S; apply Nat.le_refl).
+                                rewrite <- n_adder_cout_bexp_equiv_1; try apply Nat.le_refl.
+                                rewrite <- bexp_interpret_equiv_1.
+                                rewrite <- bexp_interpret_equiv_1.
+                                rewrite <- bexp_interpret_equiv_1.
+                                simpl. reflexivity.
+                                induction n; try reflexivity.
+                                simpl. apply IHn.
+                            + Transparent compute_adder_n. simpl.
+                              replace (n - n + (n - n) + (n - n)) with 0 in * by omega.
+                              destruct n.
+                              * simpl. reflexivity.
+                              * simpl. replace (match n with
+                                                | 0 => S n
+                                                | S l => n - l
+                                                end) with 1.
+                                replace (n - n + (n - n) + (n - n)) with 0 in * by omega.
+                                rewrite <- n_adder_cout_bexp_equiv_1; try apply Nat.le_refl.
+                                rewrite <- n_adder_cout_bexp_equiv_1; try (apply le_S; apply Nat.le_refl).
+                                rewrite <- n_adder_cout_bexp_equiv_1; try apply Nat.le_refl.
+                                rewrite <- bexp_interpret_equiv_1.
+                                rewrite <- bexp_interpret_equiv_1.
+                                rewrite <- bexp_interpret_equiv_1.
+                                simpl. reflexivity.
+                                induction n; try reflexivity.
+                                simpl. apply IHn.
+                            + simpl. reflexivity.
+                            + simpl. reflexivity.
+                            + clear l1 l2.
+                              specialize (adder_circ_n_spec_right_1 n f) as H.
+                              simpl in H. unfold ctx_to_matrix in H. simpl in H.
+                              rewrite dim_eq_lemma_2 in H. rewrite H. clear H.
+                              assert (H : forall x : Var,
+                                         (compute_adder_n_right
+                                            n (fun i : Var =>
+                                                 match i with
+                                                 | 0 =>
+                                                   compute_adder_n_left
+                                                     n (fun v : Var => f (S (S (S (S v))))) 0
+                                                 | S i' =>
+                                                   compute_adder_n_left
+                                                     n (fun v0 : Var => f (S (S (S (S v0))))) (S i')
+                                                 end) (S x))
+                                         = compute_adder_n (S n) f (S (S (S (S (S x)))))).
+                              { intros. simpl.
+                                assert (L : forall x : Var,
+                                           compute_adder_n_right
+                                             n (fun i : Var =>
+                                                  match i with
+                                                  | 0 =>
+                                                    compute_adder_n_left
+                                                      n (fun v : Var => f (S (S (S (S v))))) 0
+                                                  | S i' =>
+                                                    compute_adder_n_left
+                                                      n (fun v0 : Var =>
+                                                           f (S (S (S (S v0))))) (S i')
+                                                  end) (S x)
+                                           = compute_adder_n_right
+                                               n
+                                               (compute_adder_n_left
+                                               n (fun v0 : Var =>
+                                                    f (S (S (S (S v0)))))) (S x)).
+                                { unfold compute_adder_n_right.
+                                  destruct n.
+                                  - reflexivity.
+                                  - destruct x0; try reflexivity. }
+                                rewrite L. clear L.
+
+                                generalize dependent x. generalize dependent f. induction n.
+                                - reflexivity.
+                                - intros. simpl.
+                                  destruct x; try reflexivity.
+                                  destruct x; try reflexivity.
+                                  destruct x.
+                                  + destruct n.
+                                    * reflexivity.
+                                    * reflexivity.
+                                  + destruct n.
+                                    * simpl in *. reflexivity.
+                                    * specialize (IHn (fun i => f (S (S (S i))))) as H.
+                                      simpl in *. rewrite <- H. clear H. reflexivity.
+                              }
+                              rewrite dim_eq_lemma_2. apply kron_eq_1.
+                              * destruct n; reflexivity.
+                              * apply big_kron_eq_1. simpl in *.
+                                intros. rewrite H. reflexivity.
+                          - apply WF_bool_to_matrix.
+                          - apply WF_bool_to_matrix.
+                          - apply WF_bool_to_matrix.
+                          - apply WF_bool_to_matrix.
+                        }
+                        { apply id_circ_WT. }
+                        { apply adder_circ_n_right_WT. }
+                        { show_mixed. }
+                        { repeat (try apply (mixed_kron 2); try apply mixed_big_kron; try show_mixed).
+                          specialize (mixed_state_big_kron_ctx_to_mat_list (n + (n + (n + (n + 0)))) (fun v : Var => compute_adder_n_left n (fun i : Var => f (S (S (S (S i))))) (S v))) as Hmixed.
+                          rewrite dim_eq_lemma_2 in Hmixed. simpl in Hmixed. apply Hmixed. }
+                      * apply id_circ_WT.
+                      * apply inPar_WT; try apply id_circ_WT. apply adder_circ_n_right_WT.
+                      * show_mixed.
+                      * repeat (try apply (mixed_kron 2); try apply mixed_big_kron; try show_mixed).
+                        specialize (mixed_state_big_kron_ctx_to_mat_list (n + (n + (n + (n + 0)))) (fun v : Var => compute_adder_n_left n (fun i : Var => f (S (S (S (S i))))) (S v))) as Hmixed.
+                        rewrite dim_eq_lemma_2 in Hmixed. simpl in Hmixed. apply Hmixed.
+                    + apply id_circ_WT.
+                    + repeat apply inPar_WT; try apply id_circ_WT.
+                      apply adder_circ_n_right_WT.
+                    + show_mixed.
+                    + repeat (try apply (mixed_kron 2); try apply mixed_big_kron; try show_mixed).
+                        specialize (mixed_state_big_kron_ctx_to_mat_list (n + (n + (n + (n + 0)))) (fun v : Var => compute_adder_n_left n (fun i : Var => f (S (S (S (S i))))) (S v))) as Hmixed.
+                        rewrite dim_eq_lemma_2 in Hmixed. simpl in Hmixed. apply Hmixed.
+                  - apply id_circ_WT.
+                  - repeat apply inPar_WT; try apply id_circ_WT. apply adder_circ_n_right_WT.
+                  - show_mixed.
+                  - repeat (try apply (mixed_kron 2); try apply mixed_big_kron; try show_mixed).
+                    specialize (mixed_state_big_kron_ctx_to_mat_list (n + (n + (n + (n + 0)))) (fun v : Var => compute_adder_n_left n (fun i : Var => f (S (S (S (S i))))) (S v))) as Hmixed.
+                    rewrite dim_eq_lemma_2 in Hmixed. simpl in Hmixed. apply Hmixed.
+                }
+                { apply WF_bool_to_matrix. }
+                { apply WF_bool_to_matrix. }
+                { apply WF_bool_to_matrix. }
+                { apply WF_bool_to_matrix. }
+              * apply id_circ_WT.
+              * apply adder_circ_n_left_WT.
+              * show_mixed.                
+              * repeat (try apply (mixed_kron 2); try apply mixed_big_kron; try show_mixed).
+                specialize (mixed_state_big_kron_ctx_to_mat_list (n + (n + (n + 0))) (fun v : Var => f (S (S (S (S (S v))))))) as Hmixed.
+                rewrite dim_eq_lemma_2 in Hmixed. simpl in Hmixed. apply Hmixed.
+            + apply id_circ_WT.
+            + repeat apply inPar_WT; try apply id_circ_WT. apply adder_circ_n_left_WT.
+            + show_mixed.
+            + repeat (try apply (mixed_kron 2); try apply mixed_big_kron; try show_mixed).
+              specialize (mixed_state_big_kron_ctx_to_mat_list (n + (n + (n + 0))) (fun v : Var => f (S (S (S (S (S v))))))) as Hmixed.
+              rewrite dim_eq_lemma_2 in Hmixed. simpl in Hmixed. apply Hmixed.
+          - apply id_circ_WT.
+          - repeat apply inPar_WT; try apply id_circ_WT. apply adder_circ_n_left_WT.
+          - show_mixed.
+          - repeat (try apply (mixed_kron 2); try apply mixed_big_kron; try show_mixed).
+            specialize (mixed_state_big_kron_ctx_to_mat_list (n + (n + (n + 0))) (fun v : Var => f (S (S (S (S (S v))))))) as Hmixed.
+            rewrite dim_eq_lemma_2 in Hmixed. simpl in Hmixed. apply Hmixed.
+        }
+        { apply id_circ_WT. }
+        { repeat apply inPar_WT; try apply id_circ_WT. apply adder_circ_n_left_WT. }
+        { show_mixed. }
+        { repeat (try apply (mixed_kron 2); try apply mixed_big_kron; try show_mixed).
+          specialize (mixed_state_big_kron_ctx_to_mat_list (n + (n + (n + 0))) (fun v : Var => f (S (S (S (S (S v))))))) as Hmixed.
+          rewrite dim_eq_lemma_2 in Hmixed. simpl in Hmixed. apply Hmixed.
+        }
+      * repeat apply inPar_WT; try apply id_circ_WT. apply adder_circ_n_right_WT.
+      * apply adder_circ_1_with_pads_WT.
+    + apply inSeq_WT.
+      * apply adder_circ_1_with_pads_WT.
+      * repeat (apply inPar_WT; try apply id_circ_WT).
+        apply adder_circ_n_right_WT.
+    + repeat (apply inPar_WT; try apply id_circ_WT).
+      apply adder_circ_n_left_WT.
+Qed.
+
+Close Scope matrix_scope.
+
+Close Scope nat_scope.
+
+Open Scope nat_scope.
+
+(* Unit test : 10100(2) + 11000(2) + 1(2) = 101101(2) *)
+Lemma adder_circ_n_test_10100_11000_1 :
+  ⟦adder_circ_n 5⟧ (ctx_to_matrix (list_of_Qubits 17) (list_to_function [false; false; true; true; false; false; true; false; true; false; false; false; false; false; false; false; true] false))
+  = (ctx_to_matrix (list_of_Qubits 17) (list_to_function [true; false; true; true; true; false; true; true; true; false; false; false; false; true; false; false; true] false)).
+Proof.
+  rewrite (adder_circ_n_spec_1 5).
+  apply ctx_to_matrix_eq_1.
+  repeat (try destruct x; try reflexivity).
+Qed.
+(* Unit test : 10100(2) + 11000(2) + 0(2) = 101100(2) *)
+Lemma adder_circ_n_test_10100_11000_0 :
+  ⟦adder_circ_n 5⟧ (ctx_to_matrix (list_of_Qubits 17) (list_to_function [false; false; true; true; false; false; true; false; true; false; false; false; false; false; false; false; false] false))
+  = (ctx_to_matrix (list_of_Qubits 17) (list_to_function [true; false; true; true; true; false; true; true; true; false; false; false; false; false; false; false; false] false)).
+Proof.
+  rewrite (adder_circ_n_spec_1 5).
+  apply ctx_to_matrix_eq_1.
+  repeat (try destruct x; try reflexivity).
+Qed.
+(* Unit test : 1010010100(2) + 1100011000(2) + 0(2) = 10110101100(2) *)
+Lemma adder_circ_n_test_1010010100_1100011000_0 :
+  ⟦adder_circ_n 10⟧ (ctx_to_matrix (list_of_Qubits 32) (list_to_function [false; false; true; true; false; false; true; false; true; false; false; false; false; false; false; false; false; true; true; false; false; true; false; true; false; false; false; false; false; false; false; false] false))
+  = (ctx_to_matrix (list_of_Qubits 32) (list_to_function [true; false; true; true; true; false; true; true; true; false; false; false; false; true; false; false; false; true; true; true; false; true; true; true; false; false; false; false; false; false; false; false] false)).
+Proof.
+  rewrite (adder_circ_n_spec_1 10).
+  apply ctx_to_matrix_eq_1.
+  repeat (try destruct x; try reflexivity).
+Qed.
+(* Unit test : 10100101001010010100(2) + 11000110001100011000(2) + 0(2) = 
+               101101011010110101100(2) *)
+Lemma adder_circ_n_test_10100101001010010100_11000110001100011000_0 :
+  ⟦adder_circ_n 20⟧ (ctx_to_matrix (list_of_Qubits 62) (list_to_function [false; false; true; true; false; false; true; false; true; false; false; false; false; false; false; false; false; true; true; false; false; true; false; true; false; false; false; false; false; false; false; false; true; true; false; false; true; false; true; false; false; false; false; false; false; false; false; true; true; false; false; true; false; true; false; false; false; false; false; false; false; false] false))
+  = (ctx_to_matrix (list_of_Qubits 62) (list_to_function [true; false; true; true; true; false; true; true; true; false; false; false; false; true; false; false; false; true; true; true; false; true; true; true; false; false; false; false; true; false; false; false; true; true; true; false; true; true; true; false; false; false; false; true; false; false; false; true; true; true; false; true; true; true; false; false; false; false; false; false; false; false] false)).
+Proof.
+  rewrite (adder_circ_n_spec_1 20).
+  apply ctx_to_matrix_eq_1.
+  repeat (try destruct x; try reflexivity).
+Qed.
+
+Fixpoint nat_bool_list (n : nat) (i : nat) : list bool :=
+  match i with
+  | O => (@nil bool)
+  | S i' => (Nat.odd n) :: (nat_bool_list (n/2) i')
+  end.
+
+Close Scope nat.
+
+Open Scope N_scope.
+
+Fixpoint store_input_bits (x : BinNums.N) (y : BinNums.N) (len : nat) : list bool
+  := match len with
+     | O => [false]
+     | S len' => (store_input_bits (x/2) (y/2) len')
+                   ++ [false; (N.odd x); (N.odd y)]
+  end.
+
+Fixpoint store_output_bits (sum : BinNums.N) (x : BinNums.N) (y : BinNums.N) (len : nat) : list bool
+  := match len with
+     | O => [(N.odd sum)]
+     | S len' => (store_output_bits (sum/2) (x/2) (y/2) len')
+                   ++ [(N.odd sum); (N.odd x); (N.odd y)]
+     end.
+
+Definition prepare_n_adder_input (x : BinNums.N) (y : BinNums.N) (cin : bool) (len : nat) :=
+  (fun_of_bools ((store_input_bits x y len) ++ [cin])).
+
+Definition prepare_n_adder_output (sum : BinNums.N) (x : BinNums.N) (y : BinNums.N) (cin : bool) (len : nat) :=
+  (fun_of_bools ((store_output_bits sum x y len) ++ [cin])).
+
+(* Unit test : 13 + 80 + 0 = 93, length = 9 *)
+Lemma adder_circ_n_test_13_80_false_9 :
+  let x := 13 in let y := 80 in let cin := false in let sum := 93 in let len := 9%nat in
+  ⟦adder_circ_n len⟧ (ctx_to_matrix (list_of_Qubits (2+3*len)) (prepare_n_adder_input x y cin len))
+  = (ctx_to_matrix (list_of_Qubits (2+3*len)) (prepare_n_adder_output sum x y cin len)).
+Proof.
+  intros.
+  rewrite (adder_circ_n_spec_1 len (prepare_n_adder_input x y cin len)).
+  apply ctx_to_matrix_eq_1.
+  repeat (try destruct x0; try reflexivity).
+Qed.
+(* Unit test : 1310293 + 8123900 + 0 = 9434193, length = 9 
+   buffer overflow! *)
+Lemma adder_circ_n_test_1310293_8123900_false_9 :
+  let x := 1310293 in let y := 8123900 in
+                      let cin := false in let sum := 9434193 in let len := 9%nat in
+  ⟦adder_circ_n len⟧ (ctx_to_matrix (list_of_Qubits (2+3*len)) (prepare_n_adder_input x y cin len))
+  = (ctx_to_matrix (list_of_Qubits (2+3*len)) (prepare_n_adder_output sum x y cin len)).
+Proof.
+  intros.
+  rewrite (adder_circ_n_spec_1 len (prepare_n_adder_input x y cin len)).
+  apply ctx_to_matrix_eq_1.
+  repeat (try destruct x0; try reflexivity).
+  Abort.
+(* Unit test : 1310293 + 8123900 + 0 = 9434193, length = 32 *)
+Lemma adder_circ_n_test_1310293_8123900_false_32 :
+  let x := 1310293 in let y := 8123900 in
+                      let cin := false in let sum := 9434193 in let len := 32%nat in
+  ⟦adder_circ_n len⟧ (ctx_to_matrix (list_of_Qubits (2+3*len)) (prepare_n_adder_input x y cin len))
+  = (ctx_to_matrix (list_of_Qubits (2+3*len)) (prepare_n_adder_output sum x y cin len)).
+Proof.
+  intros.
+  rewrite (adder_circ_n_spec_1 len (prepare_n_adder_input x y cin len)).
+  apply ctx_to_matrix_eq_1.
+  repeat (try destruct x0; try reflexivity).
+Qed.
+(* Unit test : 1310293123487 + 8112873462390 + 0 = 9423166585877, length = 64 *)
+Lemma adder_circ_n_test_1310293123487_8112873462390_false_64 :
+  let x := 1310293123487 in let y := 8112873462390 in
+                      let cin := false in let sum := 9423166585877 in let len := 64%nat in
+  ⟦adder_circ_n len⟧ (ctx_to_matrix (list_of_Qubits (2+3*len)) (prepare_n_adder_input x y cin len))
+  = (ctx_to_matrix (list_of_Qubits (2+3*len)) (prepare_n_adder_output sum x y cin len)).
+Proof.
+  intros.
+  rewrite (adder_circ_n_spec_1 len (prepare_n_adder_input x y cin len)).
+  apply ctx_to_matrix_eq_1.
+  repeat (try destruct x0; try reflexivity).
+Qed.
+
+Close Scope N_scope.
+
+(*
+Set Printing Implicit.
+Lemma adder_circ_n_spec : forall (n : nat) (bools : list bool) (b1 b2 : bool),
+    ⟦adder_circ_n n⟧ (bools_to_matrix bools)
+    = (bools_to_matrix (bools_to_matrix (bool_carry_n n (bool_sum_n n bools))).
+Proof.
+  induction n.
+  - intros. unfold adder_circ_n. unfold calc_id_circ.
+    unfold list_of_Qubits. remember compile_correct.
+    unfold ctx_to_matrix in e. unfold bools_to_matrix.
+    simpl in *. show_dimensions. 
+    rewrite compile_correct.
+    show_dimensions.
+    rewrite compile_correct. apply calc_id_circ_spec.
+ *)
+
+(*
 Program Fixpoint adder_circ_n (n : nat) : Box ((2+n+n+n) ⨂ Qubit) ((2+n+n+n) ⨂ Qubit) := 
   match n with
   | O => calc_id_circ
@@ -499,7 +1773,7 @@ Eval simpl in n_adder_cout_bexp 3 2.
 Eval simpl in n_adder_cout_bexp 3 1.
 Eval simpl in n_adder_cout_bexp 3 0.
 
-Definition n_adder_z_bexp (n m : nat) : bexp :=
+Definition n_adder_sum_bexp (n m : nat) : bexp :=
   match m with
   | O => b_var (1+n+n+n)%nat (* cin = b_var (1+n+n+n)%nat *)
   | S m' => let i := (n-m)%nat in
@@ -509,10 +1783,10 @@ Definition n_adder_z_bexp (n m : nat) : bexp :=
                 y = b_var (2+i+i+i)%nat *)
   end.
 
-Eval simpl in n_adder_z_bexp 3 3.
-Eval simpl in n_adder_z_bexp 3 2.
-Eval simpl in n_adder_z_bexp 3 1.
-Eval simpl in n_adder_z_bexp 3 0.
+Eval simpl in n_adder_sum_bexp 3 3.
+Eval simpl in n_adder_sum_bexp 3 2.
+Eval simpl in n_adder_sum_bexp 3 1.
+Eval simpl in n_adder_sum_bexp 3 0.
 
 Fixpoint increase_vars_by (k : nat) (b : bexp) : bexp :=
   match b with
@@ -553,9 +1827,9 @@ Proof.
     omega.
 Qed.
 
-Lemma n_adder_z_bexp_equiv_1 : forall (n m : nat),
+Lemma n_adder_sum_bexp_equiv_1 : forall (n m : nat),
     (m <= n)%nat ->
-    increase_vars_by 3%nat (n_adder_z_bexp n m) = n_adder_z_bexp (S n) m.
+    increase_vars_by 3%nat (n_adder_sum_bexp n m) = n_adder_sum_bexp (S n) m.
 Proof.
   intros. generalize dependent n.
   induction m.
@@ -569,15 +1843,15 @@ Proof.
     omega.
 Qed.
 
-Fixpoint n_adder_z_compute (n m : nat) (f : Var -> bool) : (Var -> bool) :=
+Fixpoint n_adder_sum_compute (n m : nat) (f : Var -> bool) : (Var -> bool) :=
   match m with
   | O => f
   | S m' => let i := (n-m)%nat in
             fun x => (if x =? (1+i+i+i)%nat then
-                        ((n_adder_z_compute n m' f) x)
-                        ⊕ ⌈ n_adder_z_bexp n m | (n_adder_z_compute n m' f) ⌉
+                        ((n_adder_sum_compute n m' f) x)
+                        ⊕ ⌈ n_adder_sum_bexp n m | (n_adder_sum_compute n m' f) ⌉
                      else
-                       ((n_adder_z_compute n m' f) x))
+                       ((n_adder_sum_compute n m' f) x))
   end.
 
 Definition n_adder_cout_compute (n : nat) (f : Var -> bool) : (Var -> bool) :=
@@ -586,13 +1860,17 @@ Definition n_adder_cout_compute (n : nat) (f : Var -> bool) : (Var -> bool) :=
            | S x' => f (S x')
            end.
 
-Eval compute in (n_adder_z_compute 2 2 (fun_of_bools [false; false ; true; true; false; true; true; false])) 1%nat.
-Eval compute in (n_adder_z_compute 3 3 (fun_of_bools [false; false ; true; true; false; true; true; false; true; true; true])).
+Eval compute in (n_adder_sum_compute 2 2 (fun_of_bools [false; false ; true; true; false; true; true; false])) 1%nat.
+Eval compute in (n_adder_sum_compute 3 3 (fun_of_bools [false; false ; true; true; false; true; true; false; true; true; true])).
 Eval compute in (n_adder_cout_compute 3 (fun_of_bools [false; false ; true; true; false; true; true; false; true; true; true])).
-Eval compute in (n_adder_cout_compute 3 (n_adder_z_compute 3 3 (fun_of_bools [false; false ; true; true; false; true; true; false; true; true; true]))).
+Eval compute in (n_adder_cout_compute 3 (n_adder_sum_compute 3 3 (fun_of_bools [false; false ; true; true; false; true; true; false; true; true; true]))).
 
 Open Scope matrix_scope.
-Open Scope nat_scope.
+
+Lemma adder_circ_n_spec_2 : forall (n : nat) (bools : list bool),
+    ⟦adder_circ_n n⟧ (matrix_of_bools bools)
+    = (matrix_of_bools (n_adder_cout_compute n (n_adder_sum_compute n n bools))).
+
 
 Lemma mixed_state_big_kron_ctx_to_mat_list : forall n f,  Mixed_State (⨂ ctx_to_mat_list (list_of_Qubits n) f).
 Proof.
@@ -690,8 +1968,8 @@ Proof.
         simpl. apply IHn0. }
     simpl. rewrite <- H. apply IHn.
 Qed.
-Lemma n_adder_z_compute_preserve : forall (n m : nat) (f : Var -> bool),
-    m <= n -> forall x, (x mod 3) <> 1 -> (n_adder_z_compute n m f x) = (f x).
+Lemma n_adder_sum_compute_preserve : forall (n m : nat) (f : Var -> bool),
+    m <= n -> forall x, (x mod 3) <> 1 -> (n_adder_sum_compute n m f x) = (f x).
 Proof.
   intros n m. generalize dependent n. induction m.
   - intros. simpl. reflexivity.
@@ -720,10 +1998,10 @@ Proof.
           (f1 (S (S (S (i + S i + S i))))) by (apply H; apply gt_Sn_O).
       reflexivity. apply H.
 Qed.
-Lemma n_adder_z_compute_equiv_1 : forall (n m : nat) (f : Var -> bool),
+Lemma n_adder_sum_compute_equiv_1 : forall (n m : nat) (f : Var -> bool),
     m <= n ->
-    n_adder_z_compute n m (fun x => f (3+x))
-    = (fun x => (n_adder_z_compute (S n) m f) (3+x)).
+    n_adder_sum_compute n m (fun x => f (3+x))
+    = (fun x => (n_adder_sum_compute (S n) m f) (3+x)).
 Proof.
   intros n m. generalize dependent n. induction m.
   - intros. simpl. reflexivity.
@@ -735,10 +2013,10 @@ Proof.
     replace (i + S i + S i) with (2 + i + i + i) by omega. simpl. reflexivity.
     omega. omega. omega.
 Qed.
-Lemma n_adder_z_compute_equiv_2 : forall (n m : nat) (f1 f2 : Var -> bool),
+Lemma n_adder_sum_compute_equiv_2 : forall (n m : nat) (f1 f2 : Var -> bool),
     m <= n -> f1 = (fun x => f2 (3+x)) ->
-    (n_adder_z_compute n m f1)
-    = (fun x => ((n_adder_z_compute (S n) m f2) (3+x))).
+    (n_adder_sum_compute n m f1)
+    = (fun x => ((n_adder_sum_compute (S n) m f2) (3+x))).
 Proof.
   intros n m. generalize dependent n. induction m.
   - intros. simpl. rewrite H0. reflexivity.
@@ -750,24 +2028,24 @@ Proof.
     rewrite <- bexp_interpret_equiv_1. reflexivity.
     omega. omega. apply H0.
 Qed.
-Lemma n_adder_z_compute_equiv_3 : forall n m f1 f2,
+Lemma n_adder_sum_compute_equiv_3 : forall n m f1 f2,
     m <= n ->
     (forall x, x > 0 -> f1 x = f2 (3 + x)) ->
-    forall x, x > 0 -> n_adder_z_compute n m f1 x =
-                       n_adder_z_compute n m (fun x0 : nat => f2 (3 + x0)) x.
+    forall x, x > 0 -> n_adder_sum_compute n m f1 x =
+                       n_adder_sum_compute n m (fun x0 : nat => f2 (3 + x0)) x.
 Proof.
   induction m.
   - intros. simpl. rewrite H0. reflexivity. apply H1.
   - intros. simpl. remember (n - S m) as i.
     rewrite (IHm f1 f2).
-    rewrite n_adder_cout_interpret_equiv_1 with (f1:=n_adder_z_compute n m f1)
-                    (f2:=n_adder_z_compute n m (fun x0 : nat => f2 (3+x0))).
-    rewrite (n_adder_z_compute_preserve n m f1). simpl.
-    rewrite (n_adder_z_compute_preserve n m f1). simpl.
+    rewrite n_adder_cout_interpret_equiv_1 with (f1:=n_adder_sum_compute n m f1)
+                    (f2:=n_adder_sum_compute n m (fun x0 : nat => f2 (3+x0))).
+    rewrite (n_adder_sum_compute_preserve n m f1). simpl.
+    rewrite (n_adder_sum_compute_preserve n m f1). simpl.
     destruct (x =? S (i + i + i)) eqn:Heqx.
-    + remember (n_adder_z_compute n m (fun x0 : nat => f2 (S (S (S x0)))) x).
-      rewrite (n_adder_z_compute_preserve n m (fun x0 : nat => f2 (3+x0))).
-      rewrite (n_adder_z_compute_preserve n m (fun x0 : nat => f2 (3+x0))).
+    + remember (n_adder_sum_compute n m (fun x0 : nat => f2 (S (S (S x0)))) x).
+      rewrite (n_adder_sum_compute_preserve n m (fun x0 : nat => f2 (3+x0))).
+      rewrite (n_adder_sum_compute_preserve n m (fun x0 : nat => f2 (3+x0))).
       rewrite H0. rewrite H0. simpl. reflexivity.
       all: try replace (S (S (i + i + i))) with (i + i + i + 2) by omega;
         try replace (S (S (S (i + i + i)))) with (S i + S i + S i) by omega;
@@ -789,7 +2067,7 @@ Qed.
 Lemma adder_circ_n_spec_1 : forall (n : nat) (f : Var -> bool),
     let li := list_of_Qubits (2 + 3 * n) in
     ⟦adder_circ_n n⟧ (ctx_to_matrix li f)
-    = (ctx_to_matrix li (n_adder_cout_compute n (n_adder_z_compute n n f))).
+    = (ctx_to_matrix li (n_adder_cout_compute n (n_adder_sum_compute n n f))).
 Proof.
   induction n.
   - intros.
@@ -885,20 +2163,20 @@ Proof.
                                                       | 1 => f 1
                                                       | 2 => f 2
                                                       | 3 => f 3
-                                                      | 4 => (n_adder_z_compute n n
+                                                      | 4 => (n_adder_sum_compute n n
                                                              (fun x : Var =>
                                                                 match x with
                                                                 | 0 => false
                                                                 | x => f (3+x)
                                                                 end) 0
                                                              ⊕ ⌈ n_adder_cout_bexp n n
-                                                             | n_adder_z_compute n n
+                                                             | n_adder_sum_compute n n
                                                                (fun x : Var =>
                                                                   match x with
                                                                   | 0 => false
                                                                   | _ => f (3+x)
                                                                   end) ⌉)
-                                                      | x => (n_adder_z_compute n n
+                                                      | x => (n_adder_sum_compute n n
                                                              (fun x : Var =>
                                                                 match x with
                                                                 | 0 => false
@@ -956,8 +2234,8 @@ Proof.
     all: specialize (mixed_state_big_kron_ctx_to_mat_list
                   (n+n+n) (fun v : Var => f (S (S (S (S (S v))))))) as Hmixed1.
     all: specialize (mixed_state_big_kron_ctx_to_mat_list
-                  (n+n+n) (fun v : Var => n_adder_z_compute n n f' (S (S v)))) as Hmixed2.
-    all: repeat (try unfold list_of_Qubits in *; try rewrite dim_eq_lemma_2 in *).
+                  (n+n+n) (fun v : Var => n_adder_sum_compute n n f' (S (S v)))) as Hmixed2.
+    all: repeat (try unfold list_of_Qubits in *; try rewrite dim_eq_lemma_2 in * ).
     all: repeat (try apply Hmixed1; try apply Hmixed2).
     all: clear Hmixed1 Hmixed2.
     all: hide_dimensions; try reflexivity.
@@ -965,11 +2243,11 @@ Proof.
     + unfold ctx_to_matrix. simpl.
       replace (n + S (n + S (n + 0))) with (2 + n + n + n) by omega.
       replace (n - n) with (0) by omega. simpl.
-      assert (L1 : forall n m f, n_adder_z_compute n m f 0 = f 0).
+      assert (L1 : forall n m f, n_adder_sum_compute n m f 0 = f 0).
       { intros. induction m.
         - simpl. reflexivity.
         - simpl. remember (n0 - S m + (n0 - S m) + (n0 - S m)). apply IHm. }
-      assert (L2 : forall n m f, n_adder_z_compute n m f 2 = f 2).
+      assert (L2 : forall n m f, n_adder_sum_compute n m f 2 = f 2).
       { intros. induction m.
         - simpl. reflexivity.
         - simpl. remember (n0 - S m) as n1. destruct n1.
@@ -977,7 +2255,7 @@ Proof.
           + simpl. replace (n1 + S n1 + S n1 + 1) with (3 + n1 + n1 + n1) by omega.
             simpl. rewrite IHm. replace (n1 + S n1 + S n1) with (2 + n1 + n1 + n1) by omega.
             destruct (f0 2); reflexivity. }
-      assert (L3 : forall n m f, n_adder_z_compute n m f 3 = f 3).
+      assert (L3 : forall n m f, n_adder_sum_compute n m f 3 = f 3).
       { intros. induction m.
         - simpl. reflexivity.
         - simpl. remember (n0 - S m) as n1. destruct n1.
@@ -993,23 +2271,23 @@ Proof.
       * replace (f' 0) with false by (rewrite Heqf'; reflexivity). rewrite xorb_false_l.
         rewrite <- n_adder_cout_bexp_equiv_1.
         rewrite <- bexp_interpret_equiv_1.
-        simpl. rewrite <- n_adder_z_compute_equiv_2 with (f1:=(fun x => f (3+x))) (f2:=f).
-        replace (⌈ n_adder_cout_bexp n n | n_adder_z_compute n n (fun x : nat => f (3 + x)) ⌉)
-          with (⌈ n_adder_cout_bexp n n | n_adder_z_compute n n f' ⌉).
+        simpl. rewrite <- n_adder_sum_compute_equiv_2 with (f1:=(fun x => f (3+x))) (f2:=f).
+        replace (⌈ n_adder_cout_bexp n n | n_adder_sum_compute n n (fun x : nat => f (3 + x)) ⌉)
+          with (⌈ n_adder_cout_bexp n n | n_adder_sum_compute n n f' ⌉).
         hide_dimensions.
         reflexivity.
         apply n_adder_cout_interpret_equiv_1. intros.
-        apply n_adder_z_compute_equiv_3.
+        apply n_adder_sum_compute_equiv_3.
         omega. destruct x0. intro H0; inversion H0. rewrite Heqf'. reflexivity.
         omega. omega. reflexivity. omega.
       * replace (f' 0) with false by (rewrite Heqf'; reflexivity). rewrite xorb_false_l.
         rewrite <- n_adder_cout_bexp_equiv_1.
         rewrite <- bexp_interpret_equiv_1.
-        rewrite n_adder_cout_interpret_equiv_1 with (f1:=n_adder_z_compute n n f')
-                        (f2:=fun x : Var => n_adder_z_compute (S n) n f (3 + x)).
-        replace (n_adder_z_compute (S n) n f 1) with (f 1).
+        rewrite n_adder_cout_interpret_equiv_1 with (f1:=n_adder_sum_compute n n f')
+                        (f2:=fun x : Var => n_adder_sum_compute (S n) n f (3 + x)).
+        replace (n_adder_sum_compute (S n) n f 1) with (f 1).
         reflexivity.
-        {  assert (forall n m, m < n -> n_adder_z_compute n m f 1 = f 1).
+        {  assert (forall n m, m < n -> n_adder_sum_compute n m f 1 = f 1).
            { intros n0 m. generalize dependent n0. induction m.
              - intros. simpl. reflexivity.
              - intros. simpl. apply lt_minus_O_lt in H. remember (n0 - S m) as i.
@@ -1018,8 +2296,8 @@ Proof.
                simpl in Heqi. omega. }
            rewrite H. reflexivity. omega. }
         { intros.
-          rewrite n_adder_z_compute_equiv_3 with (f1:=f') (f2:=f).
-          rewrite n_adder_z_compute_equiv_1. reflexivity.
+          rewrite n_adder_sum_compute_equiv_3 with (f1:=f') (f2:=f).
+          rewrite n_adder_sum_compute_equiv_1. reflexivity.
           omega. omega. destruct x0. intro H0; inversion H0. rewrite Heqf'. reflexivity.
           omega. }
         omega.
@@ -1027,15 +2305,15 @@ Proof.
       * reflexivity.
       * rewrite kron_1_l.
         { apply kron_eq_1.
-          { rewrite n_adder_z_compute_equiv_3 with (f1:=f') (f2:=f).
-            rewrite n_adder_z_compute_equiv_1. reflexivity.
+          { rewrite n_adder_sum_compute_equiv_3 with (f1:=f') (f2:=f).
+            rewrite n_adder_sum_compute_equiv_1. reflexivity.
             omega. omega. destruct x. intro H; inversion H. rewrite Heqf'. reflexivity.
             omega. }
           { apply big_kron_eq_1.
             intros.
             remember (S (S x)) as x'.
-            rewrite n_adder_z_compute_equiv_3 with (f1:=f') (f2:=f).
-            rewrite n_adder_z_compute_equiv_1. reflexivity.
+            rewrite n_adder_sum_compute_equiv_3 with (f1:=f') (f2:=f).
+            rewrite n_adder_sum_compute_equiv_1. reflexivity.
             omega. omega. destruct x0. intro H0; inversion H0. rewrite Heqf'. reflexivity.
             omega. }
         }
@@ -1045,132 +2323,10 @@ Proof.
           unfold ctx_to_matrix in HWF. rewrite dim_eq_lemma_1 in HWF. apply HWF. }
 Qed.
 
-Lemma adder_circ_n_spec_2 : forall (n : nat) (arg : list bool),
-    ⟦adder_circ_n n⟧ (matrix_of_bools arg)
-    = (matrix_of_bools (n_adder_cout_compute n (n_adder_z_compute n n arg))).
-
 Close Scope matrix_scope.
 Close Scope nat_scope.
+ *)
 
-Open Scope nat_scope.
-
-(* Unit test : 10100(2) + 11000(2) + 1(2) = 101101(2) *)
-Lemma adder_circ_n_test_10100_11000_1 :
-  ⟦adder_circ_n 5⟧ (ctx_to_matrix (list_of_Qubits 17) (list_to_function [false; false; true; true; false; false; true; false; true; false; false; false; false; false; false; false; true] false))
-  = (ctx_to_matrix (list_of_Qubits 17) (list_to_function [true; false; true; true; true; false; true; true; true; false; false; false; false; true; false; false; true] false)).
-Proof.
-  rewrite (adder_circ_n_spec 5).
-  apply ctx_to_matrix_eq_1.
-  repeat (try destruct x; try reflexivity).
-Qed.
-(* Unit test : 10100(2) + 11000(2) + 0(2) = 101100(2) *)
-Lemma adder_circ_n_test_10100_11000_0 :
-  ⟦adder_circ_n 5⟧ (ctx_to_matrix (list_of_Qubits 17) (list_to_function [false; false; true; true; false; false; true; false; true; false; false; false; false; false; false; false; false] false))
-  = (ctx_to_matrix (list_of_Qubits 17) (list_to_function [true; false; true; true; true; false; true; true; true; false; false; false; false; false; false; false; false] false)).
-Proof.
-  rewrite (adder_circ_n_spec 5).
-  apply ctx_to_matrix_eq_1.
-  repeat (try destruct x; try reflexivity).
-Qed.
-(* Unit test : 1010010100(2) + 1100011000(2) + 0(2) = 10110101100(2) *)
-Lemma adder_circ_n_test_1010010100_1100011000_0 :
-  ⟦adder_circ_n 10⟧ (ctx_to_matrix (list_of_Qubits 32) (list_to_function [false; false; true; true; false; false; true; false; true; false; false; false; false; false; false; false; false; true; true; false; false; true; false; true; false; false; false; false; false; false; false; false] false))
-  = (ctx_to_matrix (list_of_Qubits 32) (list_to_function [true; false; true; true; true; false; true; true; true; false; false; false; false; true; false; false; false; true; true; true; false; true; true; true; false; false; false; false; false; false; false; false] false)).
-Proof.
-  rewrite (adder_circ_n_spec 10).
-  apply ctx_to_matrix_eq_1.
-  repeat (try destruct x; try reflexivity).
-Qed.
-(* Unit test : 10100101001010010100(2) + 11000110001100011000(2) + 0(2) = 
-               101101011010110101100(2) *)
-Lemma adder_circ_n_test_10100101001010010100_11000110001100011000_0 :
-  ⟦adder_circ_n 20⟧ (ctx_to_matrix (list_of_Qubits 62) (list_to_function [false; false; true; true; false; false; true; false; true; false; false; false; false; false; false; false; false; true; true; false; false; true; false; true; false; false; false; false; false; false; false; false; true; true; false; false; true; false; true; false; false; false; false; false; false; false; false; true; true; false; false; true; false; true; false; false; false; false; false; false; false; false] false))
-  = (ctx_to_matrix (list_of_Qubits 62) (list_to_function [true; false; true; true; true; false; true; true; true; false; false; false; false; true; false; false; false; true; true; true; false; true; true; true; false; false; false; false; true; false; false; false; true; true; true; false; true; true; true; false; false; false; false; true; false; false; false; true; true; true; false; true; true; true; false; false; false; false; false; false; false; false] false)).
-Proof.
-  rewrite (adder_circ_n_spec 20).
-  apply ctx_to_matrix_eq_1.
-  repeat (try destruct x; try reflexivity).
-Qed.
-
-Fixpoint nat_bool_list (n : nat) (i : nat) : list bool :=
-  match i with
-  | O => (@nil bool)
-  | S i' => (Nat.odd n) :: (nat_bool_list (n/2) i')
-  end.
-
-Close Scope nat.
-
-Open Scope N_scope.
-
-Fixpoint store_input_bits (x : BinNums.N) (y : BinNums.N) (len : nat) : list bool
-  := match len with
-     | O => [false]
-     | S len' => (store_input_bits (x/2) (y/2) len')
-                   ++ [false; (N.odd x); (N.odd y)]
-  end.
-
-Fixpoint store_output_bits (z : BinNums.N) (x : BinNums.N) (y : BinNums.N) (len : nat) : list bool
-  := match len with
-     | O => [(N.odd z)]
-     | S len' => (store_output_bits (z/2) (x/2) (y/2) len')
-                   ++ [(N.odd z); (N.odd x); (N.odd y)]
-     end.
-
-Definition prepare_n_adder_input (x : BinNums.N) (y : BinNums.N) (cin : bool) (len : nat) :=
-  (fun_of_bools ((store_input_bits x y len) ++ [cin])).
-
-Definition prepare_n_adder_output (z : BinNums.N) (x : BinNums.N) (y : BinNums.N) (cin : bool) (len : nat) :=
-  (fun_of_bools ((store_output_bits z x y len) ++ [cin])).
-
-(* Unit test : 13 + 80 + 0 = 93, length = 9 *)
-Lemma adder_circ_n_test_13_80_false_9 :
-  let x := 13 in let y := 80 in let cin := false in let z := 93 in let len := 9%nat in
-  ⟦adder_circ_n len⟧ (ctx_to_matrix (list_of_Qubits (2+3*len)) (prepare_n_adder_input x y cin len))
-  = (ctx_to_matrix (list_of_Qubits (2+3*len)) (prepare_n_adder_output z x y cin len)).
-Proof.
-  intros.
-  rewrite (adder_circ_n_spec len (prepare_n_adder_input x y cin len)).
-  apply ctx_to_matrix_eq_1.
-  repeat (try destruct x0; try reflexivity).
-Qed.
-(* Unit test : 1310293 + 8123900 + 0 = 9434193, length = 9 *)
-Lemma adder_circ_n_test_1310293_8123900_false_9 :
-  let x := 1310293 in let y := 8123900 in
-                      let cin := false in let z := 9434193 in let len := 9%nat in
-  ⟦adder_circ_n len⟧ (ctx_to_matrix (list_of_Qubits (2+3*len)) (prepare_n_adder_input x y cin len))
-  = (ctx_to_matrix (list_of_Qubits (2+3*len)) (prepare_n_adder_output z x y cin len)).
-Proof.
-  intros.
-  rewrite (adder_circ_n_spec len (prepare_n_adder_input x y cin len)).
-  apply ctx_to_matrix_eq_1.
-  repeat (try destruct x0; try reflexivity).
-  Abort.
-(* Unit test : 1310293 + 8123900 + 0 = 9434193, length = 32 *)
-Lemma adder_circ_n_test_1310293_8123900_false_32 :
-  let x := 1310293 in let y := 8123900 in
-                      let cin := false in let z := 9434193 in let len := 32%nat in
-  ⟦adder_circ_n len⟧ (ctx_to_matrix (list_of_Qubits (2+3*len)) (prepare_n_adder_input x y cin len))
-  = (ctx_to_matrix (list_of_Qubits (2+3*len)) (prepare_n_adder_output z x y cin len)).
-Proof.
-  intros.
-  rewrite (adder_circ_n_spec len (prepare_n_adder_input x y cin len)).
-  apply ctx_to_matrix_eq_1.
-  repeat (try destruct x0; try reflexivity).
-Qed.
-(* Unit test : 1310293123487 + 8112873462390 + 0 = 9423166585877, length = 64 *)
-Lemma adder_circ_n_test_1310293123487_8112873462390_false_64 :
-  let x := 1310293123487 in let y := 8112873462390 in
-                      let cin := false in let z := 9423166585877 in let len := 64%nat in
-  ⟦adder_circ_n len⟧ (ctx_to_matrix (list_of_Qubits (2+3*len)) (prepare_n_adder_input x y cin len))
-  = (ctx_to_matrix (list_of_Qubits (2+3*len)) (prepare_n_adder_output z x y cin len)).
-Proof.
-  intros.
-  rewrite (adder_circ_n_spec len (prepare_n_adder_input x y cin len)).
-  apply ctx_to_matrix_eq_1.
-  repeat (try destruct x0; try reflexivity).
-Qed.
-
-Close Scope N_scope.
 
 (*
 (* Simplified, but I can't see this doing what we want *)
@@ -1184,7 +2340,7 @@ Fixpoint adder_circ_n' (n : nat) : Box ((2+n) ⨂ Qubit) ((2+n) ⨂ Qubit) :=
 Open Scope matrix_scope.
 Lemma adder_circ_n'_spec : forall (n : nat) (f : Var -> bool),
 ⟦adder_circ_n' n⟧ (ctx_to_matrix (list_of_Qubits (2+n)) f)
-= (ctx_to_matrix (list_of_Qubits (2+n)) (n_adder_cout_compute n (n_adder_z_compute n n f))).
+= (ctx_to_matrix (list_of_Qubits (2+n)) (n_adder_cout_compute n (n_adder_sum_compute n n f))).
 Proof.
   induction n.
   - intros f. apply calc_id_circ_spec.
@@ -1213,7 +2369,7 @@ Abort.
 Open Scope matrix_scope.
 Lemma adder_circ_n_spec : forall (n : nat) (f : Var -> bool),
 ⟦adder_circ_n n⟧ (ctx_to_matrix (list_of_Qubits (2+n+n+n)) f)
-= (ctx_to_matrix (list_of_Qubits (2+n+n+n)) (n_adder_cout_compute n (n_adder_z_compute n n f))).
+= (ctx_to_matrix (list_of_Qubits (2+n+n+n)) (n_adder_cout_compute n (n_adder__compute n n f))).
 Proof.
   induction n.
   - intros.
